clean up Superposition_Calculus

thys/Superposition_Calculus/Clausal_Calculus_Extra.thy
@@ -1,6 +1,6 @@
 theory Clausal_Calculus_Extra
   imports
-    "Saturation_Framework_Extensions.Clausal_Calculus"
+    Saturation_Framework_Extensions.Clausal_Calculus
     Uprod_Extra
 begin
 
@@ -13,8 +13,8 @@ lemma map_literal_comp:
   using literal.map_comp
   unfolding comp_def.
 
-lemma literals_distinct [simp]: "Neg \<noteq> Pos" "Pos \<noteq> Neg"
-  by(metis literal.distinct(1))+
+lemma literals_distinct [simp]: "Pos \<noteq> Neg" "Neg \<noteq> Pos"
+  by (metis literal.distinct(1))+
 
 primrec mset_lit :: "'a uprod literal \<Rightarrow> 'a multiset" where
   "mset_lit (Pos A) = mset_uprod A" |
@@ -36,4 +36,103 @@ lemma true_lit_uprod_iff_true_lit_prod[simp]:
   unfolding true_lit_simps uprod_mem_image_iff_prod_mem[OF \<open>sym I\<close>]
   by simp_all
 
+abbreviation Pos_Upair (infix "\<approx>" 66) where
+  "Pos_Upair x y \<equiv> Pos (Upair x y)"
+
+abbreviation Neg_Upair (infix "!\<approx>" 66) where
+  "Neg_Upair x y \<equiv> Neg (Upair x y)"
+
+lemma exists_literal_for_atom [intro]: "\<exists>l. a \<in> set_literal l"
+  by (meson literal.set_intros(1))
+
+lemma exists_literal_for_term [intro]: "\<exists>l. t \<in># mset_lit l"
+  by (metis exists_uprod mset_lit.simps(1) set_mset_mset_uprod)
+
+lemma finite_set_literal [intro]: "\<And>l. finite (set_literal l)"
+  unfolding set_literal_atm_of
+  by simp
+
+lemma map_literal_map_uprod_cong: 
+  assumes "\<And>t. t \<in># mset_lit l \<Longrightarrow> f t = g t"  
+  shows "map_literal (map_uprod f) l = map_literal (map_uprod g) l"
+  using assms
+  by(cases l)(auto cong: uprod.map_cong0)
+
+lemma set_mset_set_uprod: "set_mset (mset_lit l) = set_uprod (atm_of l)"
+  by(cases l) simp_all
+
+lemma mset_lit_set_literal: "t \<in># mset_lit l \<longleftrightarrow> t \<in> \<Union>(set_uprod ` set_literal l)"
+  unfolding set_literal_atm_of
+  by(simp add: set_mset_set_uprod)
+
+lemma inj_mset_lit: "inj mset_lit"
+proof(unfold inj_def, intro allI impI)
+  fix l l' :: "'a uprod literal"
+  assume mset_lit: "mset_lit l = mset_lit l'"
+  
+  show "l = l'"
+  proof(cases l)
+    case l: (Pos a)
+    show ?thesis
+    proof(cases l')
+      case l': (Pos a')
+
+      show ?thesis
+        using mset_lit inj_mset_uprod
+        unfolding l l' inj_def
+        by auto
+    next
+      case l': (Neg a')
+
+      show ?thesis
+        using mset_lit mset_uprod_plus_neq
+        unfolding l l' 
+        by auto
+    qed
+  next
+    case l: (Neg a)
+    then show ?thesis
+     proof(cases l')
+      case l': (Pos a')
+
+      show ?thesis
+        using mset_lit mset_uprod_plus_neq
+        unfolding l l'
+        by (metis mset_lit.simps)
+    next
+      case l': (Neg a')
+
+      show ?thesis
+        using mset_lit inj_mset_plus_same inj_mset_uprod
+        unfolding l l' inj_def
+        by auto
+    qed
+  qed
+qed
+
+global_interpretation literal_functor: finite_natural_functor where
+  map = map_literal and to_set = set_literal
+  by
+    unfold_locales 
+    (auto simp: literal.map_comp literal.map_ident literal.set_map intro: literal.map_cong)
+
+global_interpretation literal_functor: natural_functor_conversion where 
+  map = map_literal and to_set = set_literal and map_to = map_literal and map_from = map_literal and 
+  map' = map_literal and to_set' = set_literal
+  by unfold_locales
+    (auto simp: literal.set_map Clausal_Logic.literal.map_comp)
+
+abbreviation uprod_literal_to_set where "uprod_literal_to_set l \<equiv> set_mset (mset_lit l)"
+
+abbreviation map_uprod_literal where "map_uprod_literal f \<equiv> map_literal (map_uprod f)"
+
+global_interpretation uprod_literal_functor: finite_natural_functor where 
+  map = map_uprod_literal and to_set = uprod_literal_to_set
+  by unfold_locales (auto simp: mset_lit_image_mset intro: map_literal_map_uprod_cong)
+
+global_interpretation uprod_literal_functor: natural_functor_conversion where 
+  map = map_uprod_literal and to_set = uprod_literal_to_set and map_to = map_uprod_literal and 
+  map_from = map_uprod_literal and map' = map_uprod_literal and to_set' = uprod_literal_to_set
+  by unfold_locales (auto simp: mset_lit_image_mset)
+ 
 end
