thys/Superposition_Calculus/Functional_Substitution_Lifting.thy
@@ -1,0 +1,465 @@
+theory Functional_Substitution_Lifting
+  imports Functional_Substitution Natural_Magma_Functor
+begin
+
+locale functional_substitution_lifting =
+  sub: functional_substitution where subst = sub_subst and vars = sub_vars +
+  natural_functor where map = map and to_set = to_set
+  for
+    sub_vars :: "'sub \<Rightarrow> 'var set" and
+    sub_subst :: "'sub \<Rightarrow> ('var \<Rightarrow> 'base) \<Rightarrow> 'sub" and
+    map :: "('sub \<Rightarrow> 'sub) \<Rightarrow> 'expr \<Rightarrow> 'expr" and
+    to_set :: "'expr \<Rightarrow> 'sub set"
+begin
+
+definition vars :: "'expr \<Rightarrow> 'var set" where
+  "vars expr \<equiv> \<Union> (sub_vars ` to_set expr)"
+
+notation sub_subst (infixl "\<cdot>\<^sub>s" 70)
+
+definition subst :: "'expr \<Rightarrow> ('var \<Rightarrow> 'base) \<Rightarrow> 'expr" (infixl "\<cdot>" 70) where
+  "expr \<cdot> \<sigma> \<equiv> map (\<lambda>sub. sub \<cdot>\<^sub>s \<sigma>) expr"
+
+lemma map_id_cong [simp]:
+  assumes "\<And>sub. sub \<in> to_set expr \<Longrightarrow> f sub = sub"
+  shows "map f expr = expr"
+  using assms
+  by simp
+
+lemma to_set_map_not_ident:
+  assumes "sub \<in> to_set expr" "f sub \<notin> to_set expr"
+  shows "map f expr \<noteq> expr"
+  using assms
+  by (metis rev_image_eqI to_set_map)
+
+lemma subst_in_to_set_subst [intro]:
+  assumes "sub \<in> to_set expr"
+  shows "sub \<cdot>\<^sub>s \<sigma> \<in> to_set (expr \<cdot> \<sigma>)"
+  unfolding subst_def to_set_map
+  using assms
+  by simp
+
+sublocale functional_substitution where subst = "(\<cdot>)" and vars = vars
+proof unfold_locales
+  fix expr \<sigma>\<^sub>1 \<sigma>\<^sub>2
+
+  show "expr \<cdot> (\<sigma>\<^sub>1 \<odot> \<sigma>\<^sub>2) = expr \<cdot> \<sigma>\<^sub>1 \<cdot> \<sigma>\<^sub>2"
+    unfolding subst_def map_comp comp_apply sub.subst_comp_subst
+    ..
+next
+  fix expr
+  show "expr \<cdot> id_subst = expr"
+    using map_ident
+    unfolding subst_def sub.subst_id_subst.
+next
+  fix expr
+  assume "vars expr = {}"
+  then show "\<forall>\<sigma>. expr \<cdot> \<sigma> = expr"
+    unfolding vars_def subst_def
+    by simp
+next
+  fix expr and \<sigma>\<^sub>1 \<sigma>\<^sub>2 :: "'var \<Rightarrow> 'base"
+  assume "\<And>var. var \<in> vars expr \<Longrightarrow> \<sigma>\<^sub>1 var = \<sigma>\<^sub>2 var"
+
+  then show "expr \<cdot> \<sigma>\<^sub>1 = expr \<cdot> \<sigma>\<^sub>2"
+    unfolding vars_def subst_def
+    using map_cong sub.subst_eq
+    by (meson UN_I)
+qed
+
+lemma ground_subst_iff_sub_ground_subst [simp]: "is_ground_subst \<gamma> \<longleftrightarrow> sub.is_ground_subst \<gamma>"
+proof(unfold is_ground_subst_def sub.is_ground_subst_def, intro iffI allI)
+  fix sub
+  assume all_ground: "\<forall>expr. is_ground (expr \<cdot> \<gamma>)"
+  show "sub.is_ground (sub \<cdot>\<^sub>s \<gamma>)"
+  proof(rule ccontr)
+    assume sub_not_ground: "\<not>sub.is_ground (sub \<cdot>\<^sub>s \<gamma>)"
+
+    then obtain expr where "sub \<in> to_set expr"
+      using exists_functor by blast
+
+    then have "\<not>is_ground (expr \<cdot> \<gamma>)"
+      using sub_not_ground to_set_map
+      unfolding subst_def vars_def
+      by auto
+
+    then show False
+      using all_ground
+      by blast
+  qed
+next
+  fix expr
+  assume "\<forall>sub. sub.is_ground (sub \<cdot>\<^sub>s \<gamma>)"
+
+  then show "is_ground (expr \<cdot> \<gamma>)"
+    unfolding vars_def subst_def
+    using to_set_map
+    by simp
+qed
+
+lemma to_set_is_ground [intro]:
+  assumes "sub \<in> to_set expr" "is_ground expr"
+  shows "sub.is_ground sub"
+  using assms
+  by (simp add: vars_def)
+
+lemma to_set_is_ground_subst:
+  assumes "sub \<in> to_set expr" "is_ground (expr \<cdot> \<gamma>)"
+  shows "sub.is_ground (sub \<cdot>\<^sub>s \<gamma>)"
+  using assms
+  by (meson subst_in_to_set_subst to_set_is_ground)
+
+lemma subst_empty:
+  assumes "to_set expr' = {}"
+  shows "expr \<cdot> \<sigma> = expr' \<longleftrightarrow> expr = expr'"
+  using assms map_id_cong to_set_map
+  unfolding subst_def
+  by (metis empty_iff image_is_empty)
+
+lemma empty_is_ground:
+  assumes "to_set expr = {}"
+  shows "is_ground expr"
+  using assms
+  by (simp add: vars_def)
+
+lemma to_set_image: "to_set (expr \<cdot> \<sigma>) = (\<lambda>a. a \<cdot>\<^sub>s \<sigma>) ` to_set expr"
+  unfolding subst_def to_set_map..
+
+lemma to_set_subset_vars_subset:
+  assumes "to_set expr \<subseteq> to_set expr'"
+  shows "vars expr \<subseteq> vars expr'"
+  using assms
+  unfolding vars_def
+  by blast
+
+lemma to_set_subset_is_ground:
+  assumes "to_set expr' \<subseteq> to_set expr" "is_ground expr"
+  shows "is_ground expr'"
+  using assms to_set_subset_vars_subset by blast
+
+end
+
+locale based_functional_substitution_lifting =
+  functional_substitution_lifting +
+  base: base_functional_substitution where subst = base_subst and vars = base_vars +
+  sub: based_functional_substitution where subst = sub_subst and vars = sub_vars
+begin
+
+sublocale based_functional_substitution where subst = subst and vars = vars
+proof unfold_locales
+  fix \<gamma>
+
+  show "is_ground_subst \<gamma> = base.is_ground_subst \<gamma>"
+    using ground_subst_iff_sub_ground_subst sub.ground_subst_iff_base_ground_subst
+    by blast
+next
+  fix expr \<rho>
+
+  show "vars (expr \<cdot> \<rho>) = \<Union> (base_vars ` \<rho> ` vars expr)"
+    using sub.vars_subst
+    unfolding subst_def vars_def
+    by simp
+qed
+
+end
+
+locale finite_variables_lifting =
+  sub: finite_variables where vars = "sub_vars :: 'sub \<Rightarrow> 'var set" and subst = sub_subst +
+  finite_natural_functor where to_set = "to_set :: 'expr \<Rightarrow> 'sub set" +
+  functional_substitution_lifting
+begin
+
+abbreviation to_fset :: "'expr \<Rightarrow> 'sub fset" where
+  "to_fset expr \<equiv>  Abs_fset (to_set expr)"
+
+sublocale finite_variables where vars = vars and subst = subst
+  by unfold_locales (auto simp: vars_def finite_to_set)
+
+lemma fset_to_fset [simp]: "fset (to_fset expr) = to_set expr"
+  using Abs_fset_inverse finite_to_set
+  by blast
+
+lemma to_fset_map: "to_fset (map f expr) = f |`| to_fset expr"
+  using to_set_map
+  by (metis fset.set_map fset_inverse fset_to_fset)
+
+lemma to_fset_is_ground_subst:
+  assumes "sub |\<in>| to_fset expr" "is_ground (subst expr \<gamma>)"
+  shows "sub.is_ground (sub \<cdot>\<^sub>s \<gamma>)"
+  using assms
+  by (simp add: to_set_is_ground_subst)
+
+end
+
+locale renaming_variables_lifting =
+  functional_substitution_lifting +
+  sub: renaming_variables where vars = sub_vars and subst = sub_subst
+begin
+
+sublocale renaming_variables where subst = subst and vars = vars
+proof unfold_locales
+  fix expr \<rho>
+  assume "sub.is_renaming \<rho>"
+
+  then show "id_subst ` vars (expr \<cdot> \<rho>) = \<rho> ` vars expr"
+    using sub.renaming_variables
+    unfolding vars_def subst_def to_set_map
+    by fastforce
+qed (rule sub.is_renaming_iff)
+
+end
+
+locale variables_in_base_imgu_lifting =
+  based_functional_substitution_lifting +
+  sub: variables_in_base_imgu where vars = sub_vars and subst = sub_subst
+begin
+
+sublocale variables_in_base_imgu where subst = subst and vars = vars
+proof unfold_locales
+  fix expr \<mu> unifications
+  assume imgu:
+    "base.is_imgu \<mu> unifications"
+    "finite unifications"
+    "\<forall>unification \<in> unifications. finite unification"
+
+  show "vars (expr \<cdot> \<mu>) \<subseteq> vars expr \<union> \<Union> (base_vars ` \<Union> unifications)"
+    using sub.variables_in_base_imgu[OF imgu]
+    unfolding vars_def subst_def to_set_map
+    by auto
+qed
+
+end
+
+locale grounding_lifting =
+  functional_substitution_lifting where sub_vars = sub_vars and sub_subst = sub_subst and
+  map = map +
+  sub: grounding where vars = sub_vars and subst = sub_subst and to_ground = sub_to_ground and
+  from_ground = sub_from_ground +
+  natural_functor_conversion where map = map and map_to = to_ground_map and
+  map_from = from_ground_map and map' = ground_map and to_set' = to_set_ground
+  for
+    sub_to_ground :: "'sub \<Rightarrow> 'sub\<^sub>G" and
+    sub_from_ground :: "'sub\<^sub>G \<Rightarrow> 'sub" and
+    sub_vars :: "'sub \<Rightarrow> 'var set" and
+    sub_subst :: "'sub \<Rightarrow> ('var \<Rightarrow> 'base) \<Rightarrow> 'sub" and
+    map :: "('sub \<Rightarrow> 'sub) \<Rightarrow> 'expr \<Rightarrow> 'expr" and
+    to_ground_map :: "('sub \<Rightarrow> 'sub\<^sub>G) \<Rightarrow> 'expr \<Rightarrow> 'expr\<^sub>G" and
+    from_ground_map :: "('sub\<^sub>G \<Rightarrow> 'sub) \<Rightarrow> 'expr\<^sub>G \<Rightarrow> 'expr" and
+    ground_map :: "('sub\<^sub>G \<Rightarrow> 'sub\<^sub>G) \<Rightarrow> 'expr\<^sub>G \<Rightarrow> 'expr\<^sub>G" and
+    to_set_ground :: "'expr\<^sub>G \<Rightarrow> 'sub\<^sub>G set"
+begin
+
+definition to_ground :: "'expr \<Rightarrow> 'expr\<^sub>G" where
+  "to_ground expr \<equiv> to_ground_map sub_to_ground expr"
+
+definition from_ground :: "'expr\<^sub>G \<Rightarrow> 'expr" where
+  "from_ground expr\<^sub>G \<equiv> from_ground_map sub_from_ground expr\<^sub>G"
+
+sublocale grounding
+  where vars = vars and subst = subst and to_ground = to_ground and from_ground = from_ground
+proof unfold_locales
+
+  {
+    fix expr
+
+    assume "is_ground expr"
+
+    then have "\<forall>sub\<in>to_set expr. sub \<in> range sub_from_ground"
+      by (simp add: sub.is_ground_iff_range_from_ground vars_def)
+
+    then have "\<forall>sub\<in>to_set expr. \<exists>sub\<^sub>G. sub_from_ground sub\<^sub>G = sub"
+      by fast
+
+    then have "\<exists>expr\<^sub>G. from_ground expr\<^sub>G = expr"
+      unfolding from_ground_def
+      by (metis conversion_map_comp map_id_cong)
+
+    then have "expr \<in> range from_ground"
+      unfolding from_ground_def
+      by blast
+  }
+
+  moreover {
+    fix expr var
+
+    assume "var \<in> vars (from_ground expr)"
+
+    then have False
+      unfolding vars_def from_ground_def
+      using sub.ground_is_ground to_set_map_from by auto
+  }
+
+  ultimately show "{expr. is_ground expr} = range from_ground"
+    by blast
+next
+  fix expr\<^sub>G
+  show "to_ground (from_ground expr\<^sub>G) = expr\<^sub>G"
+    unfolding from_ground_def to_ground_def
+    by simp
+qed
+
+lemma to_set_from_ground: "to_set (from_ground expr) = sub_from_ground ` (to_set_ground expr)"
+  unfolding from_ground_def
+  by simp
+
+lemma sub_in_ground_is_ground:
+  assumes "sub \<in> to_set (from_ground expr)"
+  shows "sub.is_ground sub"
+  using assms
+  by (simp add: to_set_is_ground)
+
+lemma ground_sub_in_ground:
+  "sub \<in> to_set_ground expr \<longleftrightarrow> sub_from_ground sub \<in> to_set (from_ground expr)"
+  by (simp add: inj_image_mem_iff sub.inj_from_ground to_set_from_ground)
+
+lemma ground_sub:
+  "(\<forall>sub \<in> to_set (from_ground expr\<^sub>G). P sub) \<longleftrightarrow>
+   (\<forall>sub\<^sub>G \<in> to_set_ground expr\<^sub>G. P (sub_from_ground sub\<^sub>G))"
+  by (simp add: to_set_from_ground)
+
+end
+
+locale all_subst_ident_iff_ground_lifting =
+  finite_variables_lifting where map = map +
+  sub: all_subst_ident_iff_ground where subst = sub_subst and vars = sub_vars
+for map :: "('sub \<Rightarrow> 'sub) \<Rightarrow> 'expr \<Rightarrow> 'expr"
+begin
+
+sublocale all_subst_ident_iff_ground where subst = subst and vars = vars
+proof unfold_locales
+  fix expr
+
+  show "is_ground expr \<longleftrightarrow> (\<forall>\<sigma>. expr \<cdot> \<sigma> = expr)"
+  proof(rule iffI allI)
+    assume "is_ground expr"
+    then show "\<forall>\<sigma>. expr \<cdot> \<sigma> = expr"
+      by simp
+  next
+    assume all_subst_ident: "\<forall>\<sigma>. expr \<cdot> \<sigma> = expr"
+
+    show "is_ground expr"
+    proof(rule ccontr)
+      assume "\<not>is_ground expr"
+
+      then obtain sub where sub: "sub \<in> to_set expr" "\<not>sub.is_ground sub"
+        unfolding vars_def
+        by blast
+
+      then obtain \<sigma> where "sub \<cdot>\<^sub>s \<sigma> \<noteq> sub" and "sub \<cdot>\<^sub>s \<sigma> \<notin> to_set expr"
+        using sub.exists_non_ident_subst finite_to_set
+        by blast
+
+      then show False
+        using sub subst_in_to_set_subst all_subst_ident
+        by metis
+    qed
+  qed
+next
+  fix expr :: 'expr and S :: "'expr set"
+
+  assume finite: "finite S" and not_ground: "\<not>is_ground expr"
+
+  then have finite_subs: "finite (\<Union>(to_set ` insert expr S))"
+    using finite_to_set by blast
+
+  obtain sub where sub: "sub \<in> to_set expr" and sub_not_ground: "\<not>sub.is_ground sub"
+    using not_ground
+    unfolding vars_def
+    by blast
+
+  obtain \<sigma> where \<sigma>_not_ident: "sub \<cdot>\<^sub>s \<sigma> \<noteq> sub" "sub \<cdot>\<^sub>s \<sigma> \<notin> \<Union> (to_set ` insert expr S)"
+    using sub.exists_non_ident_subst[OF finite_subs sub_not_ground]
+    by blast
+
+  then have "expr \<cdot> \<sigma> \<noteq> expr"
+    using sub
+    unfolding subst_def
+    by (simp add: to_set_map_not_ident)
+
+  moreover have "expr \<cdot> \<sigma> \<notin> S"
+    using \<sigma>_not_ident(2) sub to_set_map
+    unfolding subst_def
+    by auto
+
+  ultimately show "\<exists>\<sigma>. expr \<cdot> \<sigma> \<noteq> expr \<and> expr \<cdot> \<sigma> \<notin> S"
+    by blast
+qed
+
+end
+
+locale natural_magma_functional_substitution_lifting =
+  functional_substitution_lifting + natural_magma
+begin
+
+lemma vars_add [simp]:
+  "vars (add sub expr) = sub_vars sub \<union> vars expr"
+  unfolding vars_def
+  using to_set_add by auto
+
+lemma vars_plus [simp]:
+  "vars (plus expr expr') = vars expr \<union> vars expr'"
+  unfolding vars_def
+  by (simp add: to_set_plus)
+
+lemma is_ground_add [simp]:
+  "is_ground (add sub expr) \<longleftrightarrow> sub.is_ground sub \<and> is_ground expr"
+  using vars_add by simp
+
+end
+
+locale natural_magma_functor_functional_substitution_lifting =
+  natural_magma_functional_substitution_lifting + natural_magma_functor
+begin
+
+lemma add_subst [simp]:
+  "(add sub expr) \<cdot> \<sigma> = add (sub \<cdot>\<^sub>s \<sigma>) (expr \<cdot> \<sigma>)"
+  unfolding subst_def
+  using map_add
+  by simp
+
+lemma plus_subst [simp]: "(plus expr expr') \<cdot> \<sigma> = plus (expr \<cdot> \<sigma>) (expr' \<cdot> \<sigma>)"
+  unfolding subst_def
+  using map_plus
+  by simp
+
+end
+
+locale natural_magma_grounding_lifting =
+  grounding_lifting +
+  natural_magma_functional_substitution_lifting +
+  ground: natural_magma where
+  to_set = to_set_ground and plus = plus_ground and wrap = wrap_ground and add = add_ground
+for plus_ground wrap_ground add_ground +
+assumes
+  to_ground_plus [simp]:
+   "\<And>expr expr'. to_ground (plus expr expr') = plus_ground (to_ground expr) (to_ground expr')" and
+  wrap_from_ground: "\<And>sub. from_ground (wrap_ground sub) = wrap (sub_from_ground sub)" and
+  wrap_to_ground: "\<And>sub. to_ground (wrap sub) = wrap_ground (sub_to_ground sub)"
+begin
+
+lemma from_ground_plus [simp]:
+  "from_ground (plus_ground expr expr') = plus (from_ground expr) (from_ground expr')"
+  using to_ground_plus
+  by (metis Un_empty_left from_ground_inverse ground_is_ground to_ground_inverse vars_plus)
+
+lemma from_ground_add [simp]:
+  "from_ground (add_ground sub expr) = add (sub_from_ground sub) (from_ground expr)"
+  unfolding ground.add_def add_def
+  using from_ground_plus
+  by (simp add: wrap_from_ground)
+
+lemma to_ground_add [simp]:
+  "to_ground (add sub expr) = add_ground (sub_to_ground sub) (to_ground expr)"
+  unfolding ground.add_def add_def
+  using from_ground_add wrap_to_ground
+  by simp
+
+lemma ground_add:
+  assumes "from_ground expr = add sub expr'"
+  shows "expr = add_ground (sub_to_ground sub) (to_ground expr')"
+  using assms
+  by (metis from_ground_inverse to_ground_add)
+
+end
+
+end
