thys/Superposition_Calculus/Ground_Term_Extra.thy
@@ -5,4 +5,7 @@ begin
 lemma gterm_is_fun: "is_Fun (term_of_gterm t)"
   by(cases t) simp
 
+no_notation subst_compose (infixl "\<circ>\<^sub>s" 75)
+no_notation subst_apply_term (infixl "\<cdot>" 67)
+
 end
