thys/Superposition_Calculus/Natural_Magma.thy
@@ -1,0 +1,23 @@
+theory Natural_Magma
+  imports Main
+begin
+
+locale natural_magma =
+  fixes
+    to_set :: "'b \<Rightarrow> 'a set" and
+    plus :: "'b \<Rightarrow> 'b \<Rightarrow> 'b" and
+    wrap :: "'a \<Rightarrow> 'b" and
+    add
+  defines "\<And>a b. add a b \<equiv> plus (wrap a) b"
+  assumes
+    to_set_plus: "\<And>b b'. to_set (plus b b') = (to_set b) \<union> (to_set b')" and
+    to_set_wrap: "\<And>a. to_set (wrap a) = {a}"
+begin
+
+lemma to_set_add: "\<And>a b. to_set (add a b) = insert a (to_set b)"
+  using to_set_plus to_set_wrap add_def
+  by simp
+
+end
+
+end
