thys/Superposition_Calculus/Superposition_Completeness.thy
@@ -1,0 +1,1836 @@
+theory Superposition_Completeness
+  imports
+    Ground_Superposition_Completeness
+    Grounded_Superposition
+    Nonground_Entailment
+    Superposition_Welltypedness_Preservation
+begin
+
+section \<open>Completeness\<close>
+
+context grounded_superposition_calculus
+begin
+
+subsection \<open>Liftings\<close>
+
+lemma eq_resolution_lifting:
+  fixes
+    D\<^sub>G C\<^sub>G :: "'f ground_atom clause" and
+    D C :: "('f, 'v) atom clause" and
+    \<gamma> :: "('f, 'v) subst"
+  defines
+    [simp]: "D\<^sub>G \<equiv> clause.to_ground (D \<cdot> \<gamma>)" and
+    [simp]: "C\<^sub>G \<equiv> clause.to_ground (C \<cdot> \<gamma>)"
+  assumes
+    ground_eq_resolution: "ground.eq_resolution D\<^sub>G C\<^sub>G" and
+    D_grounding: "clause.is_ground (D \<cdot> \<gamma>)" and 
+    C_grounding: "clause.is_ground (C \<cdot> \<gamma>)" and
+    select: "clause.from_ground (select\<^sub>G D\<^sub>G) = (select D) \<cdot> \<gamma>" and
+    D_is_welltyped: "clause.is_welltyped \<V> D" and
+    \<gamma>_is_welltyped: "is_welltyped_on (clause.vars D) \<V> \<gamma>" and
+    \<V>: "infinite_variables_per_type \<V>"
+  obtains C'
+  where
+    "eq_resolution (D, \<V>) (C', \<V>)"
+    "Infer [D\<^sub>G] C\<^sub>G \<in> inference_groundings (Infer [(D, \<V>)] (C', \<V>))"
+    "C' \<cdot> \<gamma> = C \<cdot> \<gamma>"
+  using ground_eq_resolution
+proof(cases D\<^sub>G C\<^sub>G rule: ground.eq_resolution.cases)
+  case ground_eq_resolutionI: (eq_resolutionI l\<^sub>G D\<^sub>G' t\<^sub>G)
+
+  let ?select\<^sub>G_empty = "select\<^sub>G D\<^sub>G = {#}"
+  let ?select\<^sub>G_not_empty = "select\<^sub>G D\<^sub>G \<noteq> {#}"
+
+  obtain l where
+    l_\<gamma>: "l \<cdot>l \<gamma> = term.from_ground t\<^sub>G !\<approx> term.from_ground t\<^sub>G" and
+    l_in_D: "l \<in># D" and
+    l_selected: "?select\<^sub>G_not_empty \<Longrightarrow> is_maximal l (select D)" and
+    l_\<gamma>_selected: "?select\<^sub>G_not_empty \<Longrightarrow> is_maximal (l \<cdot>l \<gamma>) (select D \<cdot> \<gamma>)" and
+    l_is_maximal: "?select\<^sub>G_empty \<Longrightarrow> is_maximal l D" and
+    l_\<gamma>_is_maximal: "?select\<^sub>G_empty \<Longrightarrow> is_maximal (l \<cdot>l \<gamma>) (D \<cdot> \<gamma>)"
+  proof-
+    obtain max_l where 
+      "is_maximal max_l D" and
+      is_max_in_D_\<gamma>: "is_maximal (max_l \<cdot>l \<gamma>) (D \<cdot> \<gamma>)"
+    proof-
+      have "D \<noteq> {#}"
+        using ground_eq_resolutionI(1)
+        by auto
+
+      then show ?thesis
+        using that D_grounding obtain_maximal_literal
+        by blast
+    qed
+
+    moreover then have "max_l \<in># D"
+      unfolding is_maximal_def 
+      by blast
+
+    moreover have "max_l \<cdot>l \<gamma> = term.from_ground t\<^sub>G !\<approx> term.from_ground t\<^sub>G" if ?select\<^sub>G_empty
+    proof(rule unique_maximal_in_ground_clause[OF D_grounding is_max_in_D_\<gamma>])
+      have "ground_is_maximal l\<^sub>G D\<^sub>G"
+        using ground_eq_resolutionI(3) that
+        unfolding is_maximal_def
+        by simp
+
+      then show "is_maximal (term.from_ground t\<^sub>G !\<approx> term.from_ground t\<^sub>G) (D \<cdot> \<gamma>)"
+        using D_grounding
+        unfolding ground_eq_resolutionI(2)
+        by simp
+    qed
+
+    moreover obtain selected_l where 
+      "selected_l \<cdot>l \<gamma> = term.from_ground t\<^sub>G !\<approx> term.from_ground t\<^sub>G" and
+      "is_maximal selected_l (select D)"
+      "is_maximal (selected_l \<cdot>l \<gamma>) (select D \<cdot> \<gamma>)"
+    if ?select\<^sub>G_not_empty
+    proof-
+      have "is_maximal (term.from_ground t\<^sub>G !\<approx> term.from_ground t\<^sub>G) (select D \<cdot> \<gamma>)" 
+        if ?select\<^sub>G_not_empty
+        using ground_eq_resolutionI(3) that select
+        unfolding ground_eq_resolutionI(2)
+        by simp
+
+      then show ?thesis
+        using
+          that
+          obtain_maximal_literal[OF _ select_ground_subst[OF D_grounding]]
+          unique_maximal_in_ground_clause[OF select_ground_subst[OF D_grounding]]
+        by (metis is_maximal_not_empty clause_subst_empty)
+    qed
+
+    moreover then have "selected_l \<in># D" if ?select\<^sub>G_not_empty
+      by (meson that maximal_in_clause mset_subset_eqD select_subset)
+
+    ultimately show ?thesis
+      using that
+      by blast
+  qed
+
+  obtain C' where D: "D = add_mset l C'"
+    using multi_member_split[OF l_in_D]
+    by blast
+
+  obtain t t' where l: "l = t !\<approx> t'"
+    using l_\<gamma> obtain_from_neg_literal_subst
+    by meson
+
+  obtain \<mu> \<sigma> where \<gamma>: "\<gamma> = \<mu> \<odot> \<sigma>" and imgu: "welltyped_imgu \<V> t t' \<mu>"
+  proof-
+    have unified: "t \<cdot>t \<gamma> = t' \<cdot>t \<gamma>"
+      using l_\<gamma>
+      unfolding l
+      by simp
+
+    moreover obtain \<tau> where welltyped: "welltyped \<V> t \<tau>" "welltyped \<V> t' \<tau>"
+      using D_is_welltyped
+      unfolding D l
+      by auto
+
+    show ?thesis
+      using obtain_welltyped_imgu[OF unified welltyped] that
+      by metis
+  qed
+
+  show ?thesis
+  proof(rule that)
+
+    show eq_resolution: "eq_resolution (D, \<V>) (C' \<cdot> \<mu>, \<V>)"
+    proof (rule eq_resolutionI, rule D, rule l, rule imgu)
+      show "select D = {#} \<and> is_maximal (l \<cdot>l \<mu>) (D \<cdot> \<mu>) \<or> is_maximal (l \<cdot>l \<mu>) ((select D) \<cdot> \<mu>)"
+      proof(cases ?select\<^sub>G_empty)
+        case True
+
+        moreover have "is_maximal (l \<cdot>l \<mu>) (D \<cdot> \<mu>)"
+        proof-
+          have "l \<cdot>l \<mu> \<in># D \<cdot> \<mu>"
+            using l_in_D 
+            by blast
+
+          then show ?thesis
+            using l_\<gamma>_is_maximal[OF True] is_maximal_if_grounding_is_maximal D_grounding
+            unfolding \<gamma>
+            by simp
+        qed
+
+        ultimately show ?thesis
+          using select
+          by simp
+      next
+        case False
+
+        have "l \<cdot>l \<mu> \<in># select D \<cdot> \<mu>"
+          using l_selected[OF False] maximal_in_clause
+          by blast
+
+        then have "is_maximal (l \<cdot>l \<mu>) (select D \<cdot> \<mu>)"
+          using 
+            select_ground_subst[OF D_grounding]
+            l_\<gamma>_selected[OF False] 
+            is_maximal_if_grounding_is_maximal 
+          unfolding \<gamma>
+          by auto
+
+        then show ?thesis
+          using select
+          by blast
+      qed
+    qed (rule refl)
+
+    show C'_\<mu>_\<gamma>: "C' \<cdot> \<mu> \<cdot> \<gamma> = C \<cdot> \<gamma>"
+    proof-
+      have "term.is_idem \<mu>"
+        using imgu 
+        unfolding term_subst.is_imgu_iff_is_idem_and_is_mgu 
+        by blast  
+
+      then have \<mu>_\<gamma>: "\<mu> \<odot> \<gamma> = \<gamma>"
+        unfolding \<gamma> term_subst.is_idem_def subst_compose_assoc[symmetric]
+        by argo
+
+      have "D \<cdot> \<gamma> = add_mset (l \<cdot>l \<gamma>) (C \<cdot> \<gamma>)"
+      proof-
+        have "clause.to_ground (D \<cdot> \<gamma>) = clause.to_ground (add_mset (l \<cdot>l \<gamma>) (C \<cdot> \<gamma>))"
+          using ground_eq_resolutionI(1)
+          unfolding ground_eq_resolutionI(2) l_\<gamma> ground_eq_resolutionI(4)[symmetric]
+          by simp 
+
+        moreover have "clause.is_ground (add_mset (l \<cdot>l \<gamma>) (C \<cdot> \<gamma>))"
+          using C_grounding clause.to_set_is_ground_subst[OF l_in_D D_grounding]
+          by simp
+
+        ultimately show ?thesis
+          using clause.to_ground_eq[OF D_grounding]
+          by blast
+      qed
+
+      then have "C' \<cdot> \<gamma> = C \<cdot> \<gamma>"
+        unfolding D
+        by simp
+
+      then show ?thesis
+        unfolding clause.subst_comp_subst[symmetric] \<mu>_\<gamma>.
+    qed
+
+    show "Infer [D\<^sub>G] C\<^sub>G \<in> inference_groundings (Infer [(D, \<V>)] (C' \<cdot> \<mu>, \<V>))"
+    proof (rule is_inference_grounding_one_premise_inference_groundings)
+
+      show "is_inference_grounding_one_premise (D, \<V>) (C' \<cdot> \<mu>, \<V>) (Infer [D\<^sub>G] C\<^sub>G) \<gamma>"
+      proof(unfold split, intro conjI; (rule D_grounding D_is_welltyped refl \<V>)?)
+        show "clause.is_ground (C' \<cdot> \<mu> \<cdot> \<gamma>)"
+          using C_grounding C'_\<mu>_\<gamma>
+          by argo
+      next
+        show "Infer [D\<^sub>G] C\<^sub>G = Infer [clause.to_ground (D \<cdot> \<gamma>)] (clause.to_ground (C' \<cdot> \<mu> \<cdot> \<gamma>))"
+          using C'_\<mu>_\<gamma>
+          by simp
+      next
+        have "clause.vars (C' \<cdot> \<mu>) \<subseteq> clause.vars D"
+          using clause.variables_in_base_imgu imgu
+          unfolding D l
+          by auto
+
+        then show "is_welltyped_on (clause.vars (C' \<cdot> \<mu>)) \<V> \<gamma>"
+          using D_is_welltyped \<gamma>_is_welltyped
+          by blast
+      next
+        show "clause.is_welltyped \<V> (C' \<cdot> \<mu>)"
+          using D_is_welltyped eq_resolution eq_resolution_preserves_typing
+          by blast
+      qed
+
+      show "Infer [D\<^sub>G] C\<^sub>G \<in> ground.G_Inf"
+        unfolding ground.G_Inf_def
+        using ground_eq_resolution
+        by blast
+    qed
+  qed
+qed
+
+lemma eq_factoring_lifting:
+  fixes 
+    D\<^sub>G C\<^sub>G :: "'f ground_atom clause" and 
+    D C :: "('f, 'v) atom clause" and
+    \<gamma> :: "('f, 'v) subst"
+  defines 
+    [simp]: "D\<^sub>G \<equiv> clause.to_ground (D \<cdot> \<gamma>)" and
+    [simp]: "C\<^sub>G \<equiv> clause.to_ground (C \<cdot> \<gamma>)"
+  assumes
+    ground_eq_factoring: "ground.eq_factoring D\<^sub>G C\<^sub>G" and
+    D_grounding: "clause.is_ground (D \<cdot> \<gamma>)" and
+    C_grounding: "clause.is_ground (C \<cdot> \<gamma>)" and
+    select: "clause.from_ground (select\<^sub>G D\<^sub>G) = (select D) \<cdot> \<gamma>" and
+    D_is_welltyped: "clause.is_welltyped \<V> D" and
+    \<gamma>_is_welltyped: "is_welltyped_on (clause.vars D) \<V> \<gamma>" and
+    \<V>: "infinite_variables_per_type \<V>"
+  obtains C' 
+  where
+    "eq_factoring (D, \<V>) (C', \<V>)"
+    "Infer [D\<^sub>G] C\<^sub>G \<in> inference_groundings (Infer [(D, \<V>)] (C', \<V>))"
+    "C' \<cdot> \<gamma> = C \<cdot> \<gamma>"
+  using ground_eq_factoring
+proof(cases D\<^sub>G C\<^sub>G rule: ground.eq_factoring.cases)
+  case ground_eq_factoringI: (eq_factoringI l\<^sub>G\<^sub>1 l\<^sub>G\<^sub>2 D\<^sub>G' t\<^sub>G\<^sub>1 t\<^sub>G\<^sub>2 t\<^sub>G\<^sub>3)
+
+  have "D \<noteq> {#}"
+    using ground_eq_factoringI(1)
+    by auto
+
+  then obtain l\<^sub>1 where 
+    l\<^sub>1_is_maximal: "is_maximal l\<^sub>1 D" and
+    l\<^sub>1_\<gamma>_is_maximal: "is_maximal (l\<^sub>1 \<cdot>l \<gamma>) (D \<cdot> \<gamma>)"
+    using that obtain_maximal_literal D_grounding
+    by blast
+
+  obtain t\<^sub>1 t\<^sub>1' where
+    l\<^sub>1: "l\<^sub>1 = t\<^sub>1 \<approx> t\<^sub>1'" and
+    l\<^sub>1_\<gamma>: "l\<^sub>1 \<cdot>l \<gamma> = term.from_ground t\<^sub>G\<^sub>1 \<approx> term.from_ground t\<^sub>G\<^sub>2" and
+    t\<^sub>1_\<gamma>: "t\<^sub>1 \<cdot>t \<gamma> = term.from_ground t\<^sub>G\<^sub>1" and
+    t\<^sub>1'_\<gamma>: "t\<^sub>1' \<cdot>t \<gamma> = term.from_ground t\<^sub>G\<^sub>2"
+  proof-
+    have "is_maximal (literal.from_ground l\<^sub>G\<^sub>1) (D \<cdot> \<gamma>)"
+      using ground_eq_factoringI(5) D_grounding
+      by simp
+
+    then have "l\<^sub>1 \<cdot>l \<gamma> = term.from_ground t\<^sub>G\<^sub>1 \<approx> term.from_ground t\<^sub>G\<^sub>2"
+      unfolding  ground_eq_factoringI(2)
+      using unique_maximal_in_ground_clause[OF D_grounding l\<^sub>1_\<gamma>_is_maximal]
+      by simp
+
+    then show ?thesis
+      using that
+      unfolding ground_eq_factoringI(2)
+      by (metis obtain_from_pos_literal_subst)
+  qed
+
+  obtain l\<^sub>2 D' where 
+    l\<^sub>2_\<gamma>: "l\<^sub>2 \<cdot>l \<gamma> = term.from_ground t\<^sub>G\<^sub>1 \<approx> term.from_ground t\<^sub>G\<^sub>3" and
+    D: "D = add_mset l\<^sub>1 (add_mset l\<^sub>2 D')"
+  proof-
+    obtain D'' where D: "D = add_mset l\<^sub>1 D''"
+      using maximal_in_clause[OF l\<^sub>1_is_maximal]
+      by (meson multi_member_split)
+
+    moreover have "D \<cdot> \<gamma> = clause.from_ground (add_mset l\<^sub>G\<^sub>1 (add_mset l\<^sub>G\<^sub>2 D\<^sub>G'))"
+      using ground_eq_factoringI(1) D\<^sub>G_def
+      by (metis D_grounding clause.to_ground_inverse)
+
+    ultimately have "D'' \<cdot> \<gamma> =  add_mset (literal.from_ground l\<^sub>G\<^sub>2) (clause.from_ground D\<^sub>G')"
+      using  l\<^sub>1_\<gamma>
+      by (simp add: ground_eq_factoringI(2))
+
+    then obtain l\<^sub>2 where "l\<^sub>2 \<cdot>l \<gamma> = term.from_ground t\<^sub>G\<^sub>1 \<approx> term.from_ground t\<^sub>G\<^sub>3" "l\<^sub>2 \<in># D''"
+      unfolding clause.subst_def ground_eq_factoringI
+      using msed_map_invR
+      by force
+
+    then show ?thesis
+      using that
+      unfolding D
+      by (metis mset_add)
+  qed
+
+  then obtain t\<^sub>2 t\<^sub>2' where 
+    l\<^sub>2: "l\<^sub>2 = t\<^sub>2 \<approx> t\<^sub>2'" and
+    t\<^sub>2_\<gamma>: "t\<^sub>2 \<cdot>t \<gamma> = term.from_ground t\<^sub>G\<^sub>1" and
+    t\<^sub>2'_\<gamma>: "t\<^sub>2' \<cdot>t \<gamma> = term.from_ground t\<^sub>G\<^sub>3"
+    unfolding ground_eq_factoringI(3) 
+    using obtain_from_pos_literal_subst
+    by metis
+
+  have D'_\<gamma>: "D' \<cdot> \<gamma> = clause.from_ground D\<^sub>G'" 
+    using D D_grounding ground_eq_factoringI(1,2,3) l\<^sub>1_\<gamma> l\<^sub>2_\<gamma> 
+    by force
+
+  obtain \<mu> \<sigma> where \<gamma>: "\<gamma> = \<mu> \<odot> \<sigma>" and imgu: "welltyped_imgu \<V> t\<^sub>1 t\<^sub>2 \<mu>"
+  proof-
+    have unified: "t\<^sub>1 \<cdot>t \<gamma> = t\<^sub>2 \<cdot>t \<gamma>"
+      unfolding t\<^sub>1_\<gamma> t\<^sub>2_\<gamma> ..
+
+    then obtain \<tau> where "welltyped \<V> (t\<^sub>1 \<cdot>t \<gamma>) \<tau>" "welltyped \<V> (t\<^sub>2 \<cdot>t \<gamma>) \<tau>"
+      using D_is_welltyped \<gamma>_is_welltyped
+      unfolding D l\<^sub>1 l\<^sub>2
+      by auto
+
+    then have welltyped: "welltyped \<V> t\<^sub>1 \<tau>" "welltyped \<V> t\<^sub>2 \<tau>"
+      using \<gamma>_is_welltyped
+      unfolding D l\<^sub>1 l\<^sub>2
+      by simp_all
+
+    then show ?thesis
+      using obtain_welltyped_imgu[OF unified welltyped] that
+      by metis
+  qed
+
+  let ?C'' = "add_mset (t\<^sub>1 \<approx> t\<^sub>2') (add_mset (t\<^sub>1' !\<approx> t\<^sub>2') D')"
+  let ?C' = "?C'' \<cdot> \<mu>"
+
+  show ?thesis
+  proof(rule that)
+
+    show eq_factoring: "eq_factoring (D, \<V>) (?C', \<V>)"
+    proof (rule eq_factoringI; (rule D l\<^sub>1 l\<^sub>2 imgu refl)?)
+      show "select D = {#}"
+        using ground_eq_factoringI(4) select
+        by simp
+    next
+      have "l\<^sub>1 \<cdot>l \<mu> \<in># D \<cdot> \<mu>"
+        using l\<^sub>1_is_maximal clause.subst_in_to_set_subst maximal_in_clause 
+        by blast
+
+      then show "is_maximal (l\<^sub>1 \<cdot>l \<mu>) (D \<cdot> \<mu>)"
+        using is_maximal_if_grounding_is_maximal D_grounding l\<^sub>1_\<gamma>_is_maximal
+        unfolding \<gamma>
+        by auto
+    next
+      have groundings: "term.is_ground (t\<^sub>1' \<cdot>t \<mu> \<cdot>t \<sigma>)" "term.is_ground (t\<^sub>1 \<cdot>t \<mu> \<cdot>t \<sigma>)"
+        using t\<^sub>1'_\<gamma> t\<^sub>1_\<gamma>
+        unfolding \<gamma>
+        by simp_all
+
+      have "t\<^sub>1' \<cdot>t \<gamma> \<prec>\<^sub>t t\<^sub>1 \<cdot>t \<gamma>"
+        using ground_eq_factoringI(6)
+        unfolding t\<^sub>1'_\<gamma> t\<^sub>1_\<gamma> term.order.less\<^sub>G_def.
+
+      then show "\<not> t\<^sub>1 \<cdot>t \<mu> \<preceq>\<^sub>t t\<^sub>1' \<cdot>t \<mu>"
+        unfolding \<gamma> 
+        using term.order.ground_less_not_less_eq[OF groundings]
+        by simp
+    qed
+
+    show C'_\<gamma>: "?C' \<cdot> \<gamma> = C \<cdot> \<gamma>"
+    proof-
+      have "term.is_idem \<mu>"
+        using imgu 
+        unfolding term_subst.is_imgu_iff_is_idem_and_is_mgu 
+        by blast  
+
+      then have \<mu>_\<gamma>: "\<mu> \<odot> \<gamma> = \<gamma>"
+        unfolding \<gamma> term_subst.is_idem_def subst_compose_assoc[symmetric]
+        by argo
+
+      have "C \<cdot> \<gamma> = clause.from_ground (add_mset (t\<^sub>G\<^sub>2 !\<approx> t\<^sub>G\<^sub>3) (add_mset (t\<^sub>G\<^sub>1 \<approx> t\<^sub>G\<^sub>3) D\<^sub>G'))"
+        using ground_eq_factoringI(7) clause.to_ground_eq[OF C_grounding clause.ground_is_ground]
+        unfolding C\<^sub>G_def
+        by (metis clause.from_ground_inverse)
+
+      also have "... = ?C'' \<cdot> \<gamma>"
+        using t\<^sub>1_\<gamma> t\<^sub>1'_\<gamma> t\<^sub>2'_\<gamma> D'_\<gamma>
+        by simp
+
+      also have "... = ?C' \<cdot> \<gamma>"
+        unfolding clause.subst_comp_subst[symmetric] \<mu>_\<gamma> ..
+
+      finally show ?thesis ..
+    qed
+
+    show "Infer [D\<^sub>G] C\<^sub>G \<in> inference_groundings (Infer [(D, \<V>)] (?C', \<V>))"
+    proof (rule is_inference_grounding_one_premise_inference_groundings)
+
+      show "is_inference_grounding_one_premise (D, \<V>) (?C', \<V>) (Infer [D\<^sub>G] C\<^sub>G) \<gamma>"
+      proof(unfold split, intro conjI; (rule D_grounding D_is_welltyped refl \<V>)?)
+        show "clause.is_ground (?C' \<cdot> \<gamma>)"
+          using C_grounding C'_\<gamma>
+          by argo
+      next
+        show "Infer [D\<^sub>G] C\<^sub>G = Infer [clause.to_ground (D \<cdot> \<gamma>)] (clause.to_ground (?C' \<cdot> \<gamma>))"
+          using C'_\<gamma>
+          by simp
+      next
+        have imgu: "term.is_imgu \<mu> {{t\<^sub>1, t\<^sub>2}}"
+          using imgu
+          by blast
+
+        have "clause.vars ?C' \<subseteq> clause.vars D"
+          using clause.variables_in_base_imgu[OF imgu, of ?C'']
+          unfolding D l\<^sub>1 l\<^sub>2
+          by auto
+
+        then show "is_welltyped_on (clause.vars ?C') \<V> \<gamma>"
+          using D_is_welltyped \<gamma>_is_welltyped
+          by blast
+      next
+        show "clause.is_welltyped \<V> ?C'"
+          using D_is_welltyped eq_factoring eq_factoring_preserves_typing
+          by blast
+      qed
+
+      show "Infer [D\<^sub>G] C\<^sub>G \<in> ground.G_Inf"
+        unfolding ground.G_Inf_def
+        using ground_eq_factoring
+        by blast
+    qed
+  qed
+qed
+
+lemma superposition_lifting:
+  fixes
+    E\<^sub>G D\<^sub>G C\<^sub>G :: "'f ground_atom clause" and
+    E D C :: "('f, 'v) atom clause" and
+    \<gamma> \<rho>\<^sub>1 \<rho>\<^sub>2 :: "('f, 'v) subst" and
+    \<V>\<^sub>1 \<V>\<^sub>2 :: "('v, 'ty) var_types"
+  defines
+    [simp]: "E\<^sub>G \<equiv> clause.to_ground (E \<cdot> \<rho>\<^sub>1 \<odot> \<gamma>)" and
+    [simp]: "D\<^sub>G \<equiv> clause.to_ground (D \<cdot> \<rho>\<^sub>2 \<odot> \<gamma>)" and
+    [simp]: "C\<^sub>G \<equiv> clause.to_ground (C \<cdot> \<gamma>)" and
+    [simp]: "N\<^sub>G \<equiv> clause_groundings (E, \<V>\<^sub>1) \<union> clause_groundings (D, \<V>\<^sub>2)" and
+    [simp]: "\<iota>\<^sub>G \<equiv> Infer [D\<^sub>G, E\<^sub>G] C\<^sub>G"
+  assumes
+    ground_superposition: "ground.superposition D\<^sub>G E\<^sub>G C\<^sub>G" and
+    \<rho>\<^sub>1: "term_subst.is_renaming \<rho>\<^sub>1" and
+    \<rho>\<^sub>2: "term_subst.is_renaming \<rho>\<^sub>2" and
+    rename_apart: "clause.vars (E \<cdot> \<rho>\<^sub>1) \<inter> clause.vars (D \<cdot> \<rho>\<^sub>2) = {}" and
+    E_grounding: "clause.is_ground (E \<cdot> \<rho>\<^sub>1 \<odot> \<gamma>)" and
+    D_grounding: "clause.is_ground (D \<cdot> \<rho>\<^sub>2 \<odot> \<gamma>)" and
+    C_grounding: "clause.is_ground (C \<cdot> \<gamma>)" and
+    select_from_E: "clause.from_ground (select\<^sub>G E\<^sub>G) = (select E) \<cdot> \<rho>\<^sub>1 \<odot> \<gamma>" and
+    select_from_D: "clause.from_ground (select\<^sub>G D\<^sub>G) = (select D) \<cdot> \<rho>\<^sub>2 \<odot> \<gamma>" and
+    E_is_welltyped: "clause.is_welltyped \<V>\<^sub>1 E" and
+    D_is_welltyped: "clause.is_welltyped \<V>\<^sub>2 D" and
+    \<rho>\<^sub>1_\<gamma>_is_welltyped: "is_welltyped_on (clause.vars E) \<V>\<^sub>1 (\<rho>\<^sub>1 \<odot> \<gamma>)" and
+    \<rho>\<^sub>2_\<gamma>_is_welltyped: "is_welltyped_on (clause.vars D) \<V>\<^sub>2 (\<rho>\<^sub>2 \<odot> \<gamma>)" and
+    \<rho>\<^sub>1_is_welltyped: "is_welltyped_on (clause.vars E) \<V>\<^sub>1 \<rho>\<^sub>1" and
+    \<rho>\<^sub>2_is_welltyped: "is_welltyped_on (clause.vars D) \<V>\<^sub>2 \<rho>\<^sub>2" and
+    \<V>\<^sub>1: "infinite_variables_per_type \<V>\<^sub>1" and
+    \<V>\<^sub>2: "infinite_variables_per_type \<V>\<^sub>2" and
+    not_redundant: "\<iota>\<^sub>G \<notin> ground.Red_I N\<^sub>G"
+  obtains C' \<V>\<^sub>3
+  where
+    "superposition (D, \<V>\<^sub>2) (E, \<V>\<^sub>1) (C', \<V>\<^sub>3)"
+    "\<iota>\<^sub>G \<in> inference_groundings (Infer [(D, \<V>\<^sub>2), (E, \<V>\<^sub>1)] (C', \<V>\<^sub>3))"
+    "C' \<cdot> \<gamma> = C \<cdot> \<gamma>"
+  using ground_superposition
+proof(cases D\<^sub>G E\<^sub>G C\<^sub>G rule: ground.superposition.cases)
+  case ground_superpositionI: (superpositionI l\<^sub>G\<^sub>1 E\<^sub>G' l\<^sub>G\<^sub>2 D\<^sub>G' \<P>\<^sub>G c\<^sub>G t\<^sub>G\<^sub>1 t\<^sub>G\<^sub>2 t\<^sub>G\<^sub>3)
+
+  have E_\<gamma>: "E \<cdot> \<rho>\<^sub>1 \<odot> \<gamma> = clause.from_ground (add_mset l\<^sub>G\<^sub>1 E\<^sub>G')"
+    using ground_superpositionI(1) 
+    unfolding E\<^sub>G_def
+    by (metis E_grounding clause.to_ground_inverse)
+
+  have D_\<gamma>: "D \<cdot> \<rho>\<^sub>2 \<odot> \<gamma> = clause.from_ground (add_mset l\<^sub>G\<^sub>2 D\<^sub>G')"
+    using ground_superpositionI(2) D\<^sub>G_def
+    by (metis D_grounding clause.to_ground_inverse)
+
+  let ?select\<^sub>G_empty = "select\<^sub>G (clause.to_ground (E \<cdot> \<rho>\<^sub>1 \<odot> \<gamma>)) = {#}"
+  let ?select\<^sub>G_not_empty = "select\<^sub>G (clause.to_ground (E \<cdot> \<rho>\<^sub>1 \<odot> \<gamma>)) \<noteq> {#}"
+
+  obtain l\<^sub>1 where
+    l\<^sub>1_\<gamma>: "l\<^sub>1 \<cdot>l \<rho>\<^sub>1 \<odot> \<gamma> = literal.from_ground l\<^sub>G\<^sub>1" and
+    l\<^sub>1_is_strictly_maximal: "\<P>\<^sub>G = Pos \<Longrightarrow> is_strictly_maximal l\<^sub>1 E" and
+    l\<^sub>1_is_maximal: "\<P>\<^sub>G = Neg \<Longrightarrow> ?select\<^sub>G_empty \<Longrightarrow> is_maximal l\<^sub>1 E" and
+    l\<^sub>1_selected: "\<P>\<^sub>G = Neg \<Longrightarrow> ?select\<^sub>G_not_empty \<Longrightarrow> is_maximal l\<^sub>1 (select E)" and
+    l\<^sub>1_in_E: "l\<^sub>1 \<in># E"
+  proof-
+
+    have E_not_empty: "E \<noteq> {#}"
+      using ground_superpositionI(1) 
+      by auto
+
+    have "is_strictly_maximal (literal.from_ground l\<^sub>G\<^sub>1) (E \<cdot> \<rho>\<^sub>1 \<odot> \<gamma>)" if "\<P>\<^sub>G = Pos"
+      using ground_superpositionI(9) that E_grounding
+      by simp
+
+    then obtain positive_l\<^sub>1 where
+      "is_strictly_maximal positive_l\<^sub>1 E"
+      "positive_l\<^sub>1 \<cdot>l \<rho>\<^sub>1 \<odot> \<gamma> = literal.from_ground l\<^sub>G\<^sub>1" 
+    if "\<P>\<^sub>G = Pos"
+      using obtain_strictly_maximal_literal[OF E_grounding]
+      by metis
+
+    moreover then have "positive_l\<^sub>1 \<in># E" if "\<P>\<^sub>G = Pos"
+      using that strictly_maximal_in_clause
+      by blast
+
+    moreover then have "is_maximal (literal.from_ground l\<^sub>G\<^sub>1) (E \<cdot> \<rho>\<^sub>1 \<odot> \<gamma>)" if ?select\<^sub>G_empty
+      using that ground_superpositionI(9) is_maximal_not_empty E_grounding
+      by auto
+
+    then obtain negative_maximal_l\<^sub>1 where
+      "is_maximal negative_maximal_l\<^sub>1 E"
+      "negative_maximal_l\<^sub>1 \<cdot>l \<rho>\<^sub>1 \<odot> \<gamma> = literal.from_ground l\<^sub>G\<^sub>1"
+    if "\<P>\<^sub>G = Neg" ?select\<^sub>G_empty
+      using
+        obtain_maximal_literal[OF E_not_empty E_grounding[folded clause.subst_comp_subst]]
+        unique_maximal_in_ground_clause[OF E_grounding[folded clause.subst_comp_subst]]
+      by metis
+
+    moreover then have "negative_maximal_l\<^sub>1 \<in># E" if "\<P>\<^sub>G = Neg" ?select\<^sub>G_empty
+      using that maximal_in_clause
+      by blast
+
+    moreover have "ground_is_maximal l\<^sub>G\<^sub>1 (select\<^sub>G E\<^sub>G)" if "\<P>\<^sub>G = Neg" ?select\<^sub>G_not_empty
+      using ground_superpositionI(9) that
+      by simp
+
+    then obtain negative_selected_l\<^sub>1 where
+      "is_maximal negative_selected_l\<^sub>1 (select E)"
+      "negative_selected_l\<^sub>1 \<cdot>l \<rho>\<^sub>1 \<odot> \<gamma> = literal.from_ground l\<^sub>G\<^sub>1" 
+    if "\<P>\<^sub>G = Neg" ?select\<^sub>G_not_empty
+      using 
+        select_from_E
+        unique_maximal_in_ground_clause
+        obtain_maximal_literal
+      unfolding E\<^sub>G_def
+      by (metis (no_types, lifting) clause.ground_is_ground clause_from_ground_empty 
+          clause_subst_empty)
+
+    moreover then have "negative_selected_l\<^sub>1 \<in># E" if "\<P>\<^sub>G = Neg" ?select\<^sub>G_not_empty 
+      using that
+      by (meson maximal_in_clause mset_subset_eqD select_subset)
+
+    ultimately show ?thesis
+      using that ground_superpositionI(9)
+      by (metis literals_distinct(1))
+  qed
+
+  obtain E' where E: "E = add_mset l\<^sub>1 E'"
+    by (meson l\<^sub>1_in_E multi_member_split)
+
+  then have E'_\<gamma>: "E' \<cdot> \<rho>\<^sub>1 \<odot> \<gamma> = clause.from_ground E\<^sub>G'"
+    using l\<^sub>1_\<gamma> E_\<gamma>
+    by auto
+
+  let ?\<P> = "if \<P>\<^sub>G = Pos then Pos else Neg"
+
+  have [simp]: "\<P>\<^sub>G \<noteq> Pos \<longleftrightarrow> \<P>\<^sub>G = Neg" "\<P>\<^sub>G \<noteq> Neg \<longleftrightarrow> \<P>\<^sub>G = Pos"
+    using ground_superpositionI(4)
+    by auto
+
+  have [simp]: "\<And>a \<sigma>. ?\<P> a \<cdot>l \<sigma> = ?\<P> (a \<cdot>a \<sigma>)"
+    by auto
+
+  have [simp]: "\<And>\<V> a. literal.is_welltyped \<V> (?\<P> a) \<longleftrightarrow> atom.is_welltyped \<V> a"
+    by(auto simp: literal_is_welltyped_iff_atm_of)
+
+  have [simp]: "\<And>a. literal.vars (?\<P> a) = atom.vars a"
+    by auto
+
+  have l\<^sub>1_\<gamma>: 
+    "l\<^sub>1 \<cdot>l \<rho>\<^sub>1 \<odot> \<gamma> = ?\<P> (Upair (context.from_ground c\<^sub>G)\<langle>term.from_ground t\<^sub>G\<^sub>1\<rangle> (term.from_ground t\<^sub>G\<^sub>2))"
+    unfolding ground_superpositionI l\<^sub>1_\<gamma>
+    by simp
+
+  obtain c\<^sub>1 t\<^sub>1 t\<^sub>1' where 
+    l\<^sub>1: "l\<^sub>1 = ?\<P> (Upair c\<^sub>1\<langle>t\<^sub>1\<rangle> t\<^sub>1')" and
+    t\<^sub>1'_\<gamma>: "t\<^sub>1' \<cdot>t \<rho>\<^sub>1 \<odot> \<gamma> = term.from_ground t\<^sub>G\<^sub>2" and
+    t\<^sub>1_\<gamma>: "t\<^sub>1 \<cdot>t \<rho>\<^sub>1 \<odot> \<gamma> = term.from_ground t\<^sub>G\<^sub>1" and
+    c\<^sub>1_\<gamma>: "c\<^sub>1 \<cdot>t\<^sub>c \<rho>\<^sub>1 \<odot> \<gamma> = context.from_ground c\<^sub>G" and
+    t\<^sub>1_is_Fun: "is_Fun t\<^sub>1"
+  proof-
+
+    obtain c\<^sub>1_t\<^sub>1 t\<^sub>1' where 
+      l\<^sub>1: "l\<^sub>1 = ?\<P> (Upair c\<^sub>1_t\<^sub>1 t\<^sub>1')" and
+      t\<^sub>1'_\<gamma>: "t\<^sub>1' \<cdot>t \<rho>\<^sub>1 \<odot> \<gamma> = term.from_ground t\<^sub>G\<^sub>2" and
+      c\<^sub>1_t\<^sub>1_\<gamma>: "c\<^sub>1_t\<^sub>1 \<cdot>t \<rho>\<^sub>1 \<odot> \<gamma> = (context.from_ground c\<^sub>G)\<langle>term.from_ground t\<^sub>G\<^sub>1\<rangle>"
+      using l\<^sub>1_\<gamma>
+      by (smt (verit) obtain_from_literal_subst)
+
+    let ?inference_into_Fun =
+      "\<exists>c\<^sub>1 t\<^sub>1. 
+        c\<^sub>1_t\<^sub>1 = c\<^sub>1\<langle>t\<^sub>1\<rangle> \<and>
+        t\<^sub>1 \<cdot>t \<rho>\<^sub>1 \<odot> \<gamma> = term.from_ground t\<^sub>G\<^sub>1 \<and>
+        c\<^sub>1 \<cdot>t\<^sub>c \<rho>\<^sub>1 \<odot> \<gamma> = context.from_ground c\<^sub>G \<and>
+        is_Fun t\<^sub>1"
+
+    have "\<not> ?inference_into_Fun \<Longrightarrow> ground.redundant_infer N\<^sub>G \<iota>\<^sub>G"
+    proof-
+      assume "\<not> ?inference_into_Fun"
+
+      with c\<^sub>1_t\<^sub>1_\<gamma>
+      obtain t\<^sub>1 c\<^sub>1 c\<^sub>G' where
+        c\<^sub>1_t\<^sub>1: "c\<^sub>1_t\<^sub>1 = c\<^sub>1\<langle>t\<^sub>1\<rangle>" and
+        t\<^sub>1_is_Var: "is_Var t\<^sub>1" and
+        c\<^sub>G: "c\<^sub>G = context.to_ground (c\<^sub>1 \<cdot>t\<^sub>c \<rho>\<^sub>1 \<odot> \<gamma>) \<circ>\<^sub>c c\<^sub>G'"
+      proof(induction c\<^sub>1_t\<^sub>1 arbitrary: c\<^sub>G thesis)
+        case (Var x)
+
+        show ?case
+        proof(rule Var.prems)
+          show "Var x = \<box>\<langle>Var x\<rangle>"
+            by simp
+
+          show "is_Var (Var x)"
+            by simp
+
+          show "c\<^sub>G = context.to_ground (\<box> \<cdot>t\<^sub>c \<rho>\<^sub>1 \<odot> \<gamma>) \<circ>\<^sub>c c\<^sub>G"
+            by (simp add: context.to_ground_def)
+        qed
+      next
+        case (Fun f ts)
+
+        have "c\<^sub>G \<noteq> \<box>"
+          using Fun.prems(2,3)
+          unfolding context.from_ground_def
+          by (metis actxt.simps(8) intp_actxt.simps(1) is_FunI)
+
+        then obtain ts\<^sub>G\<^sub>1 c\<^sub>G' ts\<^sub>G\<^sub>2 where
+          c\<^sub>G: "c\<^sub>G = More f ts\<^sub>G\<^sub>1 c\<^sub>G' ts\<^sub>G\<^sub>2"
+          using Fun.prems
+          by (cases c\<^sub>G) (auto simp: context.from_ground_def)
+
+        have
+          "map (\<lambda>t. t \<cdot>t \<rho>\<^sub>1 \<odot> \<gamma>) ts =
+            map term.from_ground ts\<^sub>G\<^sub>1 @ (context.from_ground c\<^sub>G')\<langle>term.from_ground t\<^sub>G\<^sub>1\<rangle> # 
+            map term.from_ground ts\<^sub>G\<^sub>2"
+          using Fun(3)
+          unfolding c\<^sub>G context.from_ground_def
+          by simp
+
+        moreover then obtain ts\<^sub>1 t ts\<^sub>2 where 
+          ts: "ts = ts\<^sub>1 @ t # ts\<^sub>2" and
+          ts\<^sub>1_\<gamma>: "map (\<lambda>term. term \<cdot>t \<rho>\<^sub>1 \<odot> \<gamma>) ts\<^sub>1 = map term.from_ground ts\<^sub>G\<^sub>1" and
+          ts\<^sub>2_\<gamma>: "map (\<lambda>term. term \<cdot>t \<rho>\<^sub>1 \<odot> \<gamma>) ts\<^sub>2 = map term.from_ground ts\<^sub>G\<^sub>2"            
+          by (smt append_eq_map_conv map_eq_Cons_D)
+
+        ultimately have t_\<gamma>: "t \<cdot>t \<rho>\<^sub>1 \<odot> \<gamma> = (context.from_ground c\<^sub>G')\<langle>term.from_ground t\<^sub>G\<^sub>1\<rangle>"
+          by simp
+
+        obtain t\<^sub>1 c\<^sub>1 c\<^sub>G'' where 
+          "t = c\<^sub>1\<langle>t\<^sub>1\<rangle>" and
+          "is_Var t\<^sub>1" and
+          "c\<^sub>G' = context.to_ground (c\<^sub>1 \<cdot>t\<^sub>c \<rho>\<^sub>1 \<odot> \<gamma>) \<circ>\<^sub>c c\<^sub>G''"
+        proof-
+          have "t \<in> set ts"
+            by (simp add: ts)
+
+          moreover have
+            "\<nexists>c\<^sub>1 t\<^sub>1. t = c\<^sub>1\<langle>t\<^sub>1\<rangle> \<and> 
+                t\<^sub>1 \<cdot>t \<rho>\<^sub>1 \<odot> \<gamma> = term.from_ground t\<^sub>G\<^sub>1 \<and> 
+                c\<^sub>1 \<cdot>t\<^sub>c \<rho>\<^sub>1 \<odot> \<gamma> = context.from_ground c\<^sub>G' \<and> 
+                is_Fun t\<^sub>1"
+          proof(rule notI, elim exE conjE)
+            fix c\<^sub>1 t\<^sub>1
+            assume 
+              "t = c\<^sub>1\<langle>t\<^sub>1\<rangle>" 
+              "t\<^sub>1 \<cdot>t \<rho>\<^sub>1 \<odot> \<gamma> = term.from_ground t\<^sub>G\<^sub>1" 
+              "c\<^sub>1 \<cdot>t\<^sub>c \<rho>\<^sub>1 \<odot> \<gamma> = context.from_ground c\<^sub>G'" 
+              "is_Fun t\<^sub>1"
+
+            moreover then have 
+              "Fun f ts = (More f ts\<^sub>1 c\<^sub>1 ts\<^sub>2)\<langle>t\<^sub>1\<rangle>" 
+              "(More f ts\<^sub>1 c\<^sub>1 ts\<^sub>2) \<cdot>t\<^sub>c \<rho>\<^sub>1 \<odot> \<gamma> = context.from_ground c\<^sub>G"
+              unfolding context.from_ground_def c\<^sub>G ts
+              using ts\<^sub>1_\<gamma> ts\<^sub>2_\<gamma>
+              by auto
+
+            ultimately show False
+              using Fun.prems(3)
+              by blast
+          qed
+
+          ultimately show ?thesis
+            using Fun(1) t_\<gamma> that
+            by blast
+        qed
+
+        moreover then have
+          "Fun f ts = (More f ts\<^sub>1 c\<^sub>1 ts\<^sub>2)\<langle>t\<^sub>1\<rangle>"
+          "c\<^sub>G = context.to_ground (More f ts\<^sub>1 c\<^sub>1 ts\<^sub>2 \<cdot>t\<^sub>c \<rho>\<^sub>1 \<odot> \<gamma>) \<circ>\<^sub>c c\<^sub>G''"
+          using ts\<^sub>1_\<gamma> ts\<^sub>2_\<gamma>
+          unfolding context.to_ground_def c\<^sub>G ts
+          by auto
+
+        ultimately show ?case
+          using Fun.prems(1)
+          by blast
+      qed
+
+      obtain x where t\<^sub>1_\<rho>\<^sub>1: "t\<^sub>1 \<cdot>t \<rho>\<^sub>1 = Var x"
+        using t\<^sub>1_is_Var term.id_subst_rename[OF \<rho>\<^sub>1]
+        unfolding is_Var_def
+        by auto
+
+      have \<iota>\<^sub>G_parts: 
+        "set (side_prems_of \<iota>\<^sub>G) = {D\<^sub>G}" 
+        "main_prem_of \<iota>\<^sub>G = E\<^sub>G"
+        "concl_of \<iota>\<^sub>G = C\<^sub>G"
+        by simp_all
+
+      show ?thesis
+      proof(rule ground.redundant_infer_singleton, unfold \<iota>\<^sub>G_parts, intro bexI conjI)
+
+        let ?t\<^sub>G = "(context.from_ground c\<^sub>G')\<langle>term.from_ground t\<^sub>G\<^sub>3\<rangle>"
+
+        define \<gamma>' where
+          "\<gamma>' \<equiv> \<gamma>(x := ?t\<^sub>G)"
+
+        let ?E\<^sub>G' = "clause.to_ground (E \<cdot> \<rho>\<^sub>1 \<odot> \<gamma>')"
+
+        have t\<^sub>1_\<gamma>: "t\<^sub>1 \<cdot>t \<rho>\<^sub>1 \<odot> \<gamma> = (context.from_ground c\<^sub>G')\<langle>term.from_ground t\<^sub>G\<^sub>1\<rangle>"
+        proof -
+
+          have "context.is_ground (c\<^sub>1 \<cdot>t\<^sub>c \<rho>\<^sub>1 \<odot> \<gamma>)"
+            using c\<^sub>1_t\<^sub>1_\<gamma>
+            unfolding c\<^sub>1_t\<^sub>1 context.safe_unfolds
+            by (metis context.ground_is_ground context.term_with_context_is_ground 
+                term.ground_is_ground)
+
+          then show ?thesis
+            using c\<^sub>1_t\<^sub>1_\<gamma>
+            unfolding c\<^sub>1_t\<^sub>1 c\<^sub>1_t\<^sub>1_\<gamma> c\<^sub>G
+            by auto
+        qed
+
+        have t\<^sub>1_\<gamma>': "t\<^sub>1 \<cdot>t \<rho>\<^sub>1 \<odot> \<gamma>' = (context.from_ground c\<^sub>G')\<langle>term.from_ground t\<^sub>G\<^sub>3\<rangle>"
+          unfolding \<gamma>'_def
+          using t\<^sub>1_\<rho>\<^sub>1
+          by simp
+         
+        show "?E\<^sub>G' \<in> N\<^sub>G"
+        proof-
+
+          have "?E\<^sub>G' \<in> clause_groundings (E, \<V>\<^sub>1)"
+          proof(unfold clause_groundings_def mem_Collect_eq fst_conv snd_conv, 
+              intro exI conjI E_is_welltyped \<V>\<^sub>1, 
+              rule refl)
+
+            show "clause.is_ground (E \<cdot> \<rho>\<^sub>1 \<odot> \<gamma>')"
+              unfolding \<gamma>'_def
+              using E_grounding
+              by simp
+
+            show "is_welltyped_on (clause.vars E) \<V>\<^sub>1 (\<rho>\<^sub>1 \<odot> \<gamma>')"
+            proof(intro is_welltyped_on_subst_compose \<rho>\<^sub>1_is_welltyped)
+              
+              have "welltyped \<V>\<^sub>1 ?t\<^sub>G (\<V>\<^sub>1 x)"
+              proof-
+
+                have "welltyped \<V>\<^sub>1 (context.from_ground c\<^sub>G')\<langle>term.from_ground t\<^sub>G\<^sub>1\<rangle> (\<V>\<^sub>1 x)"
+                proof-
+
+                  have "welltyped \<V>\<^sub>1 (t\<^sub>1 \<cdot>t \<rho>\<^sub>1) (\<V>\<^sub>1 x)"
+                    using t\<^sub>1_\<rho>\<^sub>1
+                    by auto
+
+                  then have "welltyped \<V>\<^sub>1 (t\<^sub>1 \<cdot>t \<rho>\<^sub>1 \<odot> \<gamma>) (\<V>\<^sub>1 x)"
+                    using \<rho>\<^sub>1_is_welltyped \<rho>\<^sub>1_\<gamma>_is_welltyped
+                    unfolding E c\<^sub>1_t\<^sub>1 l\<^sub>1 subst_compose_def
+                    by simp
+
+                  moreover have "context.is_ground (c\<^sub>1 \<cdot>t\<^sub>c \<rho>\<^sub>1 \<odot> \<gamma>)"
+                    using c\<^sub>1_t\<^sub>1_\<gamma> 
+                    unfolding c\<^sub>1_t\<^sub>1 context.safe_unfolds
+                    by (metis context.ground_is_ground context.term_with_context_is_ground 
+                        term.ground_is_ground)
+
+                  then have "t\<^sub>1 \<cdot>t \<rho>\<^sub>1 \<odot> \<gamma> = (context.from_ground c\<^sub>G')\<langle>term.from_ground t\<^sub>G\<^sub>1\<rangle>"
+                    using c\<^sub>1_t\<^sub>1_\<gamma>
+                    unfolding c\<^sub>1_t\<^sub>1 c\<^sub>1_t\<^sub>1_\<gamma> c\<^sub>G
+                    by auto
+
+                  ultimately show ?thesis
+                    by argo
+                qed
+
+                moreover obtain \<tau> where
+                  "welltyped \<V>\<^sub>1 (term.from_ground t\<^sub>G\<^sub>1) \<tau>" 
+                  "welltyped \<V>\<^sub>1 (term.from_ground t\<^sub>G\<^sub>3) \<tau>"
+                proof-
+                  have "clause.is_welltyped \<V>\<^sub>2 (clause.from_ground D\<^sub>G)"
+                    using D_is_welltyped
+                    unfolding
+                      D\<^sub>G_def
+                      clause.to_ground_inverse[OF D_grounding]
+                      clause.is_welltyped.subst_stability[OF \<rho>\<^sub>2_\<gamma>_is_welltyped].
+
+                  then obtain \<tau> where
+                    "welltyped \<V>\<^sub>2 (term.from_ground t\<^sub>G\<^sub>1) \<tau>"
+                    "welltyped \<V>\<^sub>2 (term.from_ground t\<^sub>G\<^sub>3) \<tau>"
+                    unfolding ground_superpositionI
+                    by auto
+
+                  then show ?thesis
+                    using that welltyped.explicit_replace_\<V>_iff[of _ \<V>\<^sub>2 \<V>\<^sub>1]
+                    by simp
+                qed
+
+                 ultimately show ?thesis
+                  by auto              
+              qed
+
+              moreover have "is_welltyped_on (\<Union> (term.vars ` \<rho>\<^sub>1 ` clause.vars E)) \<V>\<^sub>1 \<gamma>"
+                by (intro is_welltyped_on_subst_compose_renaming \<rho>\<^sub>1_\<gamma>_is_welltyped
+                    \<rho>\<^sub>1_is_welltyped \<rho>\<^sub>1)
+
+              ultimately show "is_welltyped_on (\<Union> (term.vars ` \<rho>\<^sub>1 ` clause.vars E)) \<V>\<^sub>1 \<gamma>'"
+                unfolding \<gamma>'_def
+                by simp
+            qed
+          qed
+
+          then show ?thesis
+            by simp
+        qed
+     
+        show "ground.G_entails {?E\<^sub>G', D\<^sub>G} {C\<^sub>G}"
+        proof(unfold ground.G_entails_def, intro allI impI)
+          fix I :: "'f gterm rel"
+          let ?I = "upair ` I"
+
+          assume 
+            refl_I: "refl I" and 
+            trans_I: "trans I" and 
+            sym_I: "sym I" and
+            compatible_with_gctxt_I: "compatible_with_gctxt I" and
+            premise: "?I \<TTurnstile>s {?E\<^sub>G', D\<^sub>G}"
+
+           then interpret clause_entailment I
+             by unfold_locales
+
+          have \<gamma>_x_is_ground: "term.is_ground (\<gamma> x)"
+            using t\<^sub>1_\<gamma> t\<^sub>1_\<rho>\<^sub>1
+            by auto
+
+          show "?I \<TTurnstile>s {C\<^sub>G}"
+          proof(cases "?I \<TTurnstile> D\<^sub>G'")
+            case True
+
+            then show ?thesis
+              unfolding ground_superpositionI
+              by auto
+          next
+            case False
+
+            then have t\<^sub>G\<^sub>1_t\<^sub>G\<^sub>3: "Upair t\<^sub>G\<^sub>1 t\<^sub>G\<^sub>3 \<in> ?I"
+              using premise sym
+              unfolding ground_superpositionI
+              by auto
+
+            have "?I \<TTurnstile>l c\<^sub>G'\<langle>t\<^sub>G\<^sub>1\<rangle>\<^sub>G \<approx> c\<^sub>G'\<langle>t\<^sub>G\<^sub>3\<rangle>\<^sub>G"
+              using upair_compatible_with_gctxtI[OF t\<^sub>G\<^sub>1_t\<^sub>G\<^sub>3]
+              by auto
+
+            then have "?I \<TTurnstile>l term.to_ground (t\<^sub>1 \<cdot>t \<rho>\<^sub>1 \<odot> \<gamma>) \<approx> term.to_ground (t\<^sub>1 \<cdot>t \<rho>\<^sub>1 \<odot> \<gamma>')"
+              unfolding t\<^sub>1_\<gamma> t\<^sub>1_\<gamma>'
+              by simp
+
+            then have "(term.to_ground (\<gamma> x), c\<^sub>G'\<langle>t\<^sub>G\<^sub>3\<rangle>\<^sub>G) \<in> I"
+              unfolding \<gamma>'_def
+              using t\<^sub>1_\<rho>\<^sub>1
+              by (auto simp: sym)
+
+            moreover have "?I \<TTurnstile> ?E\<^sub>G'"
+              using premise
+              by simp
+
+            ultimately have "?I \<TTurnstile> E\<^sub>G"
+              unfolding \<gamma>'_def
+              using
+                clause.symmetric_congruence[of _ \<gamma>, OF _ \<gamma>_x_is_ground]
+                E_grounding
+              by simp
+
+            then have "?I \<TTurnstile> add_mset (\<P>\<^sub>G (Upair c\<^sub>G\<langle>t\<^sub>G\<^sub>3\<rangle>\<^sub>G t\<^sub>G\<^sub>2)) E\<^sub>G'"
+              unfolding ground_superpositionI
+              using symmetric_literal_context_congruence[OF t\<^sub>G\<^sub>1_t\<^sub>G\<^sub>3]
+              by (cases "\<P>\<^sub>G = Pos") simp_all
+
+            then show ?thesis
+              unfolding ground_superpositionI
+              by blast
+          qed
+        qed
+
+        show "?E\<^sub>G' \<prec>\<^sub>c\<^sub>G E\<^sub>G"
+        proof-
+
+          have "\<gamma> x = t\<^sub>1 \<cdot>t \<rho>\<^sub>1 \<odot> \<gamma>"
+            using t\<^sub>1_\<rho>\<^sub>1
+            by simp
+
+          then have t\<^sub>G_smaller: "?t\<^sub>G \<prec>\<^sub>t \<gamma> x"
+            using ground_superpositionI(8)
+            unfolding t\<^sub>1_\<gamma> term.order.less\<^sub>G_def
+            by simp
+
+          have "add_mset (l\<^sub>1 \<cdot>l \<rho>\<^sub>1 \<odot> \<gamma>') (E' \<cdot> \<rho>\<^sub>1 \<odot> \<gamma>') \<prec>\<^sub>c add_mset (l\<^sub>1 \<cdot>l \<rho>\<^sub>1 \<odot> \<gamma>) (E' \<cdot> \<rho>\<^sub>1 \<odot> \<gamma>)"
+          proof(rule less\<^sub>c_add_mset)
+
+            have "x \<in> literal.vars (l\<^sub>1 \<cdot>l \<rho>\<^sub>1)"
+              unfolding l\<^sub>1 c\<^sub>1_t\<^sub>1 literal.vars_def atom.vars_def 
+              using t\<^sub>1_\<rho>\<^sub>1
+              by auto
+
+            moreover have "literal.is_ground (l\<^sub>1 \<cdot>l \<rho>\<^sub>1 \<odot> \<gamma>)"
+              using E_grounding
+              unfolding E
+              by simp
+
+            ultimately show "l\<^sub>1 \<cdot>l \<rho>\<^sub>1 \<odot> \<gamma>' \<prec>\<^sub>l l\<^sub>1 \<cdot>l \<rho>\<^sub>1 \<odot> \<gamma>"
+              unfolding \<gamma>'_def
+              using literal.order.subst_update_stability t\<^sub>G_smaller
+              by simp
+          next
+
+            have "clause.is_ground (E' \<cdot> \<rho>\<^sub>1 \<odot> \<gamma>)"
+              using E'_\<gamma>
+              by simp
+
+            then show "E' \<cdot> \<rho>\<^sub>1 \<odot> \<gamma>' \<preceq>\<^sub>c E' \<cdot> \<rho>\<^sub>1 \<odot> \<gamma>"
+              unfolding \<gamma>'_def
+              using clause.order.subst_update_stability t\<^sub>G_smaller
+              by (cases "x \<in> clause.vars (E' \<cdot> \<rho>\<^sub>1)") simp_all
+          qed
+
+          then have "E \<cdot> \<rho>\<^sub>1 \<odot> \<gamma>' \<prec>\<^sub>c E \<cdot> \<rho>\<^sub>1 \<odot> \<gamma>"
+            unfolding E
+            by simp
+
+          moreover have "clause.is_ground (E \<cdot> \<rho>\<^sub>1 \<odot> \<gamma>')"
+            unfolding \<gamma>'_def
+            using E_grounding
+            by simp
+
+          ultimately show ?thesis
+            using E_grounding
+            unfolding clause.order.less\<^sub>G_def
+            by simp
+        qed
+      qed
+    qed
+
+    then show ?thesis
+      using not_redundant ground_superposition that l\<^sub>1 t\<^sub>1'_\<gamma> c\<^sub>1_t\<^sub>1_\<gamma> 
+      unfolding ground.Red_I_def ground.G_Inf_def
+      by auto
+  qed
+
+  obtain l\<^sub>2 where 
+    l\<^sub>2_\<gamma>: "l\<^sub>2 \<cdot>l \<rho>\<^sub>2 \<odot> \<gamma> = literal.from_ground l\<^sub>G\<^sub>2" and
+    l\<^sub>2_is_strictly_maximal: "is_strictly_maximal l\<^sub>2 D"
+  proof-
+    have "is_strictly_maximal (literal.from_ground l\<^sub>G\<^sub>2) (D \<cdot> \<rho>\<^sub>2 \<odot> \<gamma>)"
+      using ground_superpositionI(11) D_grounding
+      by simp
+
+    then show ?thesis
+      using obtain_strictly_maximal_literal[OF D_grounding] that
+      by metis
+  qed
+
+  then have l\<^sub>2_in_D: "l\<^sub>2 \<in># D" 
+    using strictly_maximal_in_clause 
+    by blast
+
+  from l\<^sub>2_\<gamma> have l\<^sub>2_\<gamma>: "l\<^sub>2 \<cdot>l \<rho>\<^sub>2 \<odot> \<gamma> = term.from_ground t\<^sub>G\<^sub>1 \<approx> term.from_ground t\<^sub>G\<^sub>3"
+    unfolding ground_superpositionI
+    by simp
+
+  then obtain t\<^sub>2 t\<^sub>2' where
+    l\<^sub>2: "l\<^sub>2 = t\<^sub>2 \<approx> t\<^sub>2'" and
+    t\<^sub>2_\<gamma>: "t\<^sub>2 \<cdot>t \<rho>\<^sub>2 \<odot> \<gamma> = term.from_ground t\<^sub>G\<^sub>1" and     
+    t\<^sub>2'_\<gamma>: "t\<^sub>2' \<cdot>t \<rho>\<^sub>2 \<odot> \<gamma> = term.from_ground t\<^sub>G\<^sub>3"
+    using obtain_from_pos_literal_subst
+    by metis
+
+  obtain D' where D: "D = add_mset l\<^sub>2 D'"
+    by (meson l\<^sub>2_in_D multi_member_split)
+
+  then have D'_\<gamma>: "D' \<cdot> \<rho>\<^sub>2 \<odot> \<gamma> = clause.from_ground D\<^sub>G'"
+    using D_\<gamma> l\<^sub>2_\<gamma>
+    unfolding ground_superpositionI
+    by auto
+
+  (* TODO: inv *) 
+  define \<V>\<^sub>3 where 
+    "\<And>x. \<V>\<^sub>3 x \<equiv>
+        if x \<in> clause.vars (E \<cdot> \<rho>\<^sub>1)
+        then \<V>\<^sub>1 (inv \<rho>\<^sub>1 (Var x))
+        else \<V>\<^sub>2 (inv \<rho>\<^sub>2 (Var x))"
+
+  have \<gamma>_is_welltyped: "is_welltyped_on (clause.vars (E \<cdot> \<rho>\<^sub>1) \<union> clause.vars (D \<cdot> \<rho>\<^sub>2)) \<V>\<^sub>3 \<gamma>"
+  proof(unfold Set.ball_Un, intro conjI)
+
+    show "is_welltyped_on (clause.vars (E \<cdot> \<rho>\<^sub>1)) \<V>\<^sub>3 \<gamma>"
+      unfolding \<V>\<^sub>3_def
+      using clause.is_welltyped.renaming_grounding[OF \<rho>\<^sub>1 \<rho>\<^sub>1_\<gamma>_is_welltyped E_grounding]
+      by simp
+
+  next
+    have "\<forall>x\<in>clause.vars (D \<cdot> \<rho>\<^sub>2). \<V>\<^sub>3 x = \<V>\<^sub>2 (inv \<rho>\<^sub>2 (Var x))"
+      unfolding \<V>\<^sub>3_def
+      using rename_apart
+      by auto
+
+    then show "is_welltyped_on (clause.vars (D \<cdot> \<rho>\<^sub>2)) \<V>\<^sub>3 \<gamma>"
+      unfolding \<V>\<^sub>3_def
+      using clause.is_welltyped.renaming_grounding[OF \<rho>\<^sub>2 \<rho>\<^sub>2_\<gamma>_is_welltyped D_grounding]
+      by simp
+  qed
+
+  obtain \<mu> \<sigma> where
+    \<gamma>: "\<gamma> = \<mu> \<odot> \<sigma>" and
+    imgu: "welltyped_imgu \<V>\<^sub>3 (t\<^sub>1 \<cdot>t \<rho>\<^sub>1) (t\<^sub>2 \<cdot>t \<rho>\<^sub>2) \<mu>"
+  proof-
+
+    have unified: "t\<^sub>1 \<cdot>t \<rho>\<^sub>1 \<cdot>t \<gamma> = t\<^sub>2 \<cdot>t \<rho>\<^sub>2 \<cdot>t \<gamma>"
+      using t\<^sub>1_\<gamma> t\<^sub>2_\<gamma> 
+      by simp
+
+    obtain \<tau> where welltyped: "welltyped \<V>\<^sub>3 (t\<^sub>1 \<cdot>t \<rho>\<^sub>1) \<tau>" "welltyped \<V>\<^sub>3 (t\<^sub>2 \<cdot>t \<rho>\<^sub>2) \<tau>"
+    proof-
+      have "clause.is_welltyped \<V>\<^sub>2 (D \<cdot> \<rho>\<^sub>2 \<odot> \<gamma>)"
+        using \<rho>\<^sub>2_\<gamma>_is_welltyped D_is_welltyped
+        by (metis clause.is_welltyped.subst_stability)
+
+      then obtain \<tau> where 
+        "welltyped \<V>\<^sub>2 (term.from_ground t\<^sub>G\<^sub>1) \<tau>" 
+        unfolding D_\<gamma> ground_superpositionI
+        by auto
+
+      then have "welltyped \<V>\<^sub>3 (term.from_ground t\<^sub>G\<^sub>1) \<tau>" 
+        using welltyped.is_ground_typed
+        by (meson term.ground_is_ground welltyped.explicit_is_ground_typed)
+
+      then have "welltyped \<V>\<^sub>3 (t\<^sub>1 \<cdot>t \<rho>\<^sub>1 \<odot> \<gamma>) \<tau>" "welltyped \<V>\<^sub>3 (t\<^sub>2 \<cdot>t \<rho>\<^sub>2 \<odot> \<gamma>) \<tau>"
+        using t\<^sub>1_\<gamma> t\<^sub>2_\<gamma>
+        by presburger+
+
+      moreover have
+        "term.vars (t\<^sub>1 \<cdot>t \<rho>\<^sub>1) \<subseteq> clause.vars (E \<cdot> \<rho>\<^sub>1)"
+        "term.vars (t\<^sub>2 \<cdot>t \<rho>\<^sub>2) \<subseteq> clause.vars (D \<cdot> \<rho>\<^sub>2)"
+        unfolding E l\<^sub>1 clause.add_subst D l\<^sub>2
+        by auto
+
+      ultimately have "welltyped \<V>\<^sub>3 (t\<^sub>1 \<cdot>t \<rho>\<^sub>1) \<tau>" "welltyped \<V>\<^sub>3 (t\<^sub>2 \<cdot>t \<rho>\<^sub>2) \<tau>"
+        using \<gamma>_is_welltyped
+        by (simp_all add: subsetD)
+
+      then show ?thesis
+        using that
+        by blast
+    qed
+
+    show ?thesis
+      using obtain_welltyped_imgu[OF unified welltyped] that
+      by metis
+  qed
+
+  define C' where 
+    C': "C' = add_mset (?\<P> (Upair (c\<^sub>1 \<cdot>t\<^sub>c \<rho>\<^sub>1)\<langle>t\<^sub>2' \<cdot>t \<rho>\<^sub>2\<rangle> (t\<^sub>1' \<cdot>t \<rho>\<^sub>1))) (E' \<cdot> \<rho>\<^sub>1 + D' \<cdot> \<rho>\<^sub>2) \<cdot> \<mu>"
+
+  show ?thesis
+  proof(rule that)
+
+    show superposition: "superposition (D, \<V>\<^sub>2) (E, \<V>\<^sub>1) (C', \<V>\<^sub>3)"
+    proof(rule superpositionI, rule \<rho>\<^sub>1, rule \<rho>\<^sub>2; 
+        ((rule E D l\<^sub>1 l\<^sub>2 t\<^sub>1_is_Fun imgu rename_apart \<rho>\<^sub>1_is_welltyped \<rho>\<^sub>2_is_welltyped \<V>\<^sub>1 \<V>\<^sub>2 C')+)?)
+
+      show "?\<P> \<in> {Pos, Neg}"
+        by simp
+    next
+
+      show "\<not> E \<cdot> \<rho>\<^sub>1 \<odot> \<mu> \<preceq>\<^sub>c D \<cdot> \<rho>\<^sub>2 \<odot> \<mu>"
+      proof(rule clause.order.ground_less_not_less_eq)
+
+        show "clause.vars (D \<cdot> \<rho>\<^sub>2 \<odot> \<mu> \<cdot> \<sigma>) = {}"
+          using D_grounding
+          unfolding \<gamma>
+          by simp
+
+        show "clause.vars (E \<cdot> \<rho>\<^sub>1 \<odot> \<mu> \<cdot> \<sigma>) = {}"
+          using E_grounding
+          unfolding \<gamma>
+          by simp
+
+        show "D \<cdot> \<rho>\<^sub>2 \<odot> \<mu> \<cdot> \<sigma> \<prec>\<^sub>c E \<cdot> \<rho>\<^sub>1 \<odot> \<mu> \<cdot> \<sigma>"
+          using ground_superpositionI(3) D_grounding E_grounding
+          unfolding E\<^sub>G_def D\<^sub>G_def clause.order.less\<^sub>G_def \<gamma>
+          by simp
+      qed
+    next
+      have "select E = {#}" "is_strictly_maximal (l\<^sub>1 \<cdot>l \<rho>\<^sub>1 \<odot> \<mu>) (E \<cdot> \<rho>\<^sub>1 \<odot> \<mu>)" if "?\<P> = Pos"
+      proof -
+
+        show "select E = {#}"
+          using that ground_superpositionI(9) select_from_E
+          by fastforce
+
+        show "is_strictly_maximal (l\<^sub>1 \<cdot>l \<rho>\<^sub>1 \<odot> \<mu>) (E \<cdot> \<rho>\<^sub>1 \<odot> \<mu>)"
+        proof(rule is_strictly_maximal_if_grounding_is_strictly_maximal)
+
+          show "l\<^sub>1 \<cdot>l \<rho>\<^sub>1 \<odot> \<mu> \<in># E \<cdot> \<rho>\<^sub>1 \<odot> \<mu>"
+            using l\<^sub>1_in_E
+            by blast
+
+          show "clause.is_ground (E \<cdot> \<rho>\<^sub>1 \<odot> \<mu> \<cdot> \<sigma>)"
+            using E_grounding[unfolded \<gamma>]
+            by simp
+
+          show "is_strictly_maximal (l\<^sub>1 \<cdot>l \<rho>\<^sub>1 \<odot> \<mu> \<cdot>l \<sigma>) (E \<cdot> \<rho>\<^sub>1 \<odot> \<mu> \<cdot> \<sigma>)"
+            using that l\<^sub>1_\<gamma> E_\<gamma> ground_superpositionI(9)
+            unfolding \<gamma> ground_superpositionI
+            by fastforce
+        qed
+      qed
+
+      moreover have "select E = {#}" "is_maximal (l\<^sub>1 \<cdot>l \<rho>\<^sub>1 \<odot> \<mu>) (E \<cdot> \<rho>\<^sub>1 \<odot> \<mu>)" 
+        if "?\<P> = Neg" ?select\<^sub>G_empty
+      proof-
+        show "select E = {#}"
+          using clause_subst_empty select_from_E ground_superpositionI(9) that
+          by simp
+      next
+        show "is_maximal (l\<^sub>1 \<cdot>l \<rho>\<^sub>1 \<odot> \<mu>) (E \<cdot> \<rho>\<^sub>1 \<odot> \<mu>)"
+        proof(rule is_maximal_if_grounding_is_maximal)
+
+          show "l\<^sub>1 \<cdot>l \<rho>\<^sub>1 \<odot> \<mu> \<in># E \<cdot> \<rho>\<^sub>1 \<odot> \<mu>"
+            using l\<^sub>1_in_E
+            by blast
+        next
+
+          show "clause.is_ground (E \<cdot> \<rho>\<^sub>1 \<odot> \<mu> \<cdot> \<sigma>)"
+            using E_grounding \<gamma> 
+            by auto
+        next
+
+          show "is_maximal (l\<^sub>1 \<cdot>l \<rho>\<^sub>1 \<odot> \<mu> \<cdot>l \<sigma>) (E \<cdot> \<rho>\<^sub>1 \<odot> \<mu> \<cdot> \<sigma>) "
+            using l\<^sub>1_\<gamma> \<gamma> E_\<gamma> ground_superpositionI(5,9) is_maximal_not_empty that
+            by auto
+        qed
+      qed
+
+      moreover have "is_maximal (l\<^sub>1 \<cdot>l \<rho>\<^sub>1 \<odot> \<mu>) ((select E) \<cdot> \<rho>\<^sub>1 \<odot> \<mu>)" 
+        if "?\<P> = Neg" "\<not>?select\<^sub>G_empty"
+      proof(rule is_maximal_if_grounding_is_maximal)
+
+        show "l\<^sub>1 \<cdot>l \<rho>\<^sub>1 \<odot> \<mu> \<in># select E \<cdot> \<rho>\<^sub>1 \<odot> \<mu>"
+          using ground_superpositionI(9) l\<^sub>1_selected maximal_in_clause that 
+          by auto
+      next
+
+        show "clause.is_ground (select E \<cdot> \<rho>\<^sub>1 \<odot> \<mu> \<cdot> \<sigma>)"
+          using select_ground_subst[OF E_grounding]
+          unfolding \<gamma>
+          by simp
+      next
+        show "is_maximal (l\<^sub>1 \<cdot>l \<rho>\<^sub>1 \<odot> \<mu> \<cdot>l \<sigma>) (select E \<cdot> \<rho>\<^sub>1 \<odot> \<mu> \<cdot> \<sigma>)"
+          using \<gamma> ground_superpositionI(5,9) l\<^sub>1_\<gamma> that select_from_E 
+          by fastforce
+      qed
+
+      ultimately show "?\<P> = Pos
+              \<and> select E = {#}
+              \<and> is_strictly_maximal (l\<^sub>1 \<cdot>l \<rho>\<^sub>1 \<odot> \<mu>) (E \<cdot> \<rho>\<^sub>1 \<odot> \<mu>)
+          \<or> ?\<P> = Neg
+              \<and> (select E = {#} \<and> is_maximal (l\<^sub>1 \<cdot>l \<rho>\<^sub>1 \<odot> \<mu>) (E \<cdot> \<rho>\<^sub>1 \<odot> \<mu>)
+                 \<or> is_maximal (l\<^sub>1 \<cdot>l \<rho>\<^sub>1 \<odot> \<mu>) ((select E) \<cdot> \<rho>\<^sub>1 \<odot> \<mu>))"
+        by meson
+    next
+
+      show "select D = {#}"
+        using ground_superpositionI(10) select_from_D
+        by simp
+    next 
+
+      show "is_strictly_maximal (l\<^sub>2 \<cdot>l \<rho>\<^sub>2 \<odot> \<mu>) (D \<cdot> \<rho>\<^sub>2 \<odot> \<mu>)"
+      proof(rule is_strictly_maximal_if_grounding_is_strictly_maximal)
+
+        show "l\<^sub>2 \<cdot>l \<rho>\<^sub>2 \<odot> \<mu> \<in># D \<cdot> \<rho>\<^sub>2 \<odot> \<mu>"
+          using l\<^sub>2_in_D
+          by blast
+      next
+
+        show "clause.is_ground (D \<cdot> \<rho>\<^sub>2 \<odot> \<mu> \<cdot> \<sigma>)"
+          using D_grounding
+          unfolding \<gamma>
+          by simp
+      next
+
+        show "is_strictly_maximal (l\<^sub>2 \<cdot>l \<rho>\<^sub>2 \<odot> \<mu> \<cdot>l \<sigma>) (D \<cdot> \<rho>\<^sub>2 \<odot> \<mu> \<cdot> \<sigma>)"
+          using l\<^sub>2_\<gamma> \<gamma> D_\<gamma> ground_superpositionI(6,11) 
+          by auto
+      qed
+    next
+
+      show "\<not> c\<^sub>1\<langle>t\<^sub>1\<rangle> \<cdot>t \<rho>\<^sub>1 \<odot> \<mu> \<preceq>\<^sub>t t\<^sub>1' \<cdot>t \<rho>\<^sub>1 \<odot> \<mu>"
+      proof(rule term.order.ground_less_not_less_eq)
+
+        show "term.is_ground (t\<^sub>1' \<cdot>t \<rho>\<^sub>1 \<odot> \<mu> \<cdot>t \<sigma>)"
+          using t\<^sub>1'_\<gamma> \<gamma>
+          by simp
+      next
+
+        show "term.is_ground (c\<^sub>1\<langle>t\<^sub>1\<rangle> \<cdot>t \<rho>\<^sub>1 \<odot> \<mu> \<cdot>t \<sigma>)"
+          using t\<^sub>1_\<gamma> c\<^sub>1_\<gamma> \<gamma>
+          by simp
+      next
+
+        show "t\<^sub>1' \<cdot>t \<rho>\<^sub>1 \<odot> \<mu> \<cdot>t \<sigma> \<prec>\<^sub>t c\<^sub>1\<langle>t\<^sub>1\<rangle> \<cdot>t \<rho>\<^sub>1 \<odot> \<mu> \<cdot>t \<sigma>"
+          using ground_superpositionI(7) c\<^sub>1_\<gamma> t\<^sub>1'_\<gamma> t\<^sub>1_\<gamma>
+          unfolding term.order.less\<^sub>G_def \<gamma>
+          by auto
+      qed
+    next
+
+      show "\<not> t\<^sub>2 \<cdot>t \<rho>\<^sub>2 \<odot> \<mu> \<preceq>\<^sub>t t\<^sub>2' \<cdot>t \<rho>\<^sub>2 \<odot> \<mu>"
+      proof(rule term.order.ground_less_not_less_eq)
+
+        show "term.is_ground (t\<^sub>2' \<cdot>t \<rho>\<^sub>2 \<odot> \<mu> \<cdot>t \<sigma>)"
+          using t\<^sub>2'_\<gamma> \<gamma>
+          by simp
+      next
+
+        show "term.is_ground (t\<^sub>2 \<cdot>t \<rho>\<^sub>2 \<odot> \<mu> \<cdot>t \<sigma>)"
+          using t\<^sub>2_\<gamma> \<gamma>
+          by simp
+      next
+
+        show "t\<^sub>2' \<cdot>t \<rho>\<^sub>2 \<odot> \<mu> \<cdot>t \<sigma> \<prec>\<^sub>t t\<^sub>2 \<cdot>t \<rho>\<^sub>2 \<odot> \<mu> \<cdot>t \<sigma>"
+          using ground_superpositionI(8) t\<^sub>2_\<gamma> t\<^sub>2'_\<gamma>
+          unfolding \<gamma> term.order.less\<^sub>G_def
+          by simp
+      qed
+    next
+
+      show "\<forall>x\<in>clause.vars (E \<cdot> \<rho>\<^sub>1). \<V>\<^sub>1 (inv \<rho>\<^sub>1 (Var x)) = \<V>\<^sub>3 x"
+        unfolding \<V>\<^sub>3_def
+        by auto
+    next
+
+      show "\<forall>x\<in>clause.vars (D \<cdot> \<rho>\<^sub>2). \<V>\<^sub>2 (inv \<rho>\<^sub>2 (Var x)) = \<V>\<^sub>3 x"
+        unfolding \<V>\<^sub>3_def
+        using rename_apart
+        by auto
+    next
+
+      have "\<exists>\<tau>. welltyped \<V>\<^sub>2 t\<^sub>2 \<tau> \<and> welltyped \<V>\<^sub>2 t\<^sub>2' \<tau>"
+        using D_is_welltyped
+        unfolding D l\<^sub>2
+        by auto
+
+      then show "\<And>\<tau> \<tau>'. \<lbrakk>typed \<V>\<^sub>2 t\<^sub>2 \<tau>; typed \<V>\<^sub>2 t\<^sub>2' \<tau>'\<rbrakk> \<Longrightarrow> \<tau> = \<tau>'"
+        using term.typed_if_welltyped
+        by blast
+    qed
+
+    show C'_\<gamma>: "C' \<cdot> \<gamma> = C \<cdot> \<gamma>"
+    proof-
+
+      have "term_subst.is_idem \<mu>"
+        using imgu term.is_imgu_iff_is_idem_and_is_mgu 
+        by blast
+
+      then have \<mu>_\<gamma>: "\<mu> \<odot> \<gamma> = \<gamma>"
+        unfolding \<gamma> term_subst.is_idem_def
+        by (metis subst_compose_assoc)
+
+      have "C \<cdot> \<gamma> = 
+              add_mset 
+                (?\<P> (Upair (context.from_ground c\<^sub>G)\<langle>term.from_ground t\<^sub>G\<^sub>3\<rangle> (term.from_ground t\<^sub>G\<^sub>2)))
+                  (clause.from_ground E\<^sub>G' + clause.from_ground D\<^sub>G')"
+        using ground_superpositionI(4, 12) clause.to_ground_inverse[OF C_grounding] 
+        by auto
+
+      then show ?thesis
+        unfolding 
+          C'
+          E'_\<gamma>[symmetric] 
+          D'_\<gamma>[symmetric] 
+          t\<^sub>1'_\<gamma>[symmetric]
+          t\<^sub>2'_\<gamma>[symmetric]
+          c\<^sub>1_\<gamma>[symmetric]
+          clause.subst_comp_subst[symmetric]
+          \<mu>_\<gamma>
+        by simp
+    qed
+
+    show "\<iota>\<^sub>G \<in> inference_groundings (Infer [(D, \<V>\<^sub>2), (E, \<V>\<^sub>1)] (C', \<V>\<^sub>3))"
+    proof(rule is_inference_grounding_two_premises_inference_groundings)
+
+      show "is_inference_grounding_two_premises (D, \<V>\<^sub>2) (E, \<V>\<^sub>1) (C', \<V>\<^sub>3) \<iota>\<^sub>G \<gamma> \<rho>\<^sub>1 \<rho>\<^sub>2"
+      proof(unfold split, intro conjI; 
+          (rule \<rho>\<^sub>1 \<rho>\<^sub>2 rename_apart D_grounding E_grounding D_is_welltyped E_is_welltyped refl \<V>\<^sub>1 
+            \<V>\<^sub>2)?)
+
+        show "clause.is_ground (C' \<cdot> \<gamma>)"
+          using C_grounding C'_\<gamma>
+          by argo
+      next
+
+        show "\<iota>\<^sub>G = Infer
+                    [clause.to_ground (D \<cdot> \<rho>\<^sub>2 \<odot> \<gamma>), clause.to_ground (E \<cdot> \<rho>\<^sub>1 \<odot> \<gamma>)]
+                    (clause.to_ground (C' \<cdot> \<gamma>))"
+          using C'_\<gamma>
+          by simp
+      next
+
+        show "is_welltyped_on (clause.vars C') \<V>\<^sub>3 \<gamma>"
+        proof(rule is_welltyped_on_subset[OF \<gamma>_is_welltyped])
+
+          show "clause.vars C' \<subseteq> clause.vars (E \<cdot> \<rho>\<^sub>1) \<union> clause.vars (D \<cdot> \<rho>\<^sub>2)"
+          proof (unfold subset_eq, intro ballI)
+            fix x
+
+            have is_imgu: "term.is_imgu \<mu> {{t\<^sub>1 \<cdot>t \<rho>\<^sub>1, t\<^sub>2 \<cdot>t \<rho>\<^sub>2}}"
+              using imgu
+              by blast
+
+            assume "x \<in> clause.vars C'"
+
+            then consider
+              (t\<^sub>2') "x \<in> term.vars (t\<^sub>2' \<cdot>t \<rho>\<^sub>2 \<odot> \<mu>)" |
+              (c\<^sub>1) "x \<in> context.vars (c\<^sub>1 \<cdot>t\<^sub>c \<rho>\<^sub>1 \<odot> \<mu>)" |
+              (t\<^sub>1') "x \<in> term.vars (t\<^sub>1' \<cdot>t \<rho>\<^sub>1 \<odot> \<mu>)" |
+              (E') "x \<in> clause.vars (E' \<cdot> \<rho>\<^sub>1 \<odot> \<mu>)" |  
+              (D') "x \<in> clause.vars (D' \<cdot> \<rho>\<^sub>2 \<odot> \<mu>)"  
+              unfolding C'
+              by auto
+
+            then show "x \<in> clause.vars (E \<cdot> \<rho>\<^sub>1) \<union> clause.vars (D \<cdot> \<rho>\<^sub>2)"
+            proof cases
+              case t\<^sub>2'
+
+              then show ?thesis 
+                using term.variables_in_base_imgu[OF is_imgu] 
+                unfolding E l\<^sub>1 D l\<^sub>2
+                by auto
+            next
+              case c\<^sub>1
+
+              then show ?thesis
+                using context.variables_in_base_imgu[OF is_imgu] 
+                unfolding E l\<^sub>1 D l\<^sub>2
+                by force
+            next
+              case t\<^sub>1'
+
+              then show ?thesis
+                using term.variables_in_base_imgu[OF is_imgu]
+                unfolding E clause.add_subst l\<^sub>1 D l\<^sub>2
+                by auto
+            next
+              case E'
+
+              then show ?thesis 
+                using clause.variables_in_base_imgu[OF is_imgu]
+                unfolding E l\<^sub>1 D l\<^sub>2
+                by auto
+            next
+              case D'
+
+              then show ?thesis 
+                using clause.variables_in_base_imgu[OF is_imgu]
+                unfolding E l\<^sub>1 D l\<^sub>2
+                by auto
+            qed
+          qed
+        qed
+      next
+
+        show "clause.is_welltyped \<V>\<^sub>3 C'"
+          using superposition superposition_preserves_typing E_is_welltyped D_is_welltyped
+          by blast
+      next
+
+        have "finite {x. x \<in> clause.vars (E \<cdot> \<rho>\<^sub>1)}"
+          using clause.finite_vars
+          by simp
+
+        moreover {
+          fix \<tau>
+
+          have "infinite {x. \<V>\<^sub>2 (inv \<rho>\<^sub>2 (Var x)) = \<tau>}" 
+          proof(rule surj_infinite_set[OF term.surj_inv_renaming, OF \<rho>\<^sub>2])
+
+            show "infinite {x. \<V>\<^sub>2 x = \<tau>}"
+              using \<V>\<^sub>2
+              unfolding infinite_variables_per_type_def
+              by blast
+          qed
+        }
+
+        ultimately show "infinite_variables_per_type \<V>\<^sub>3"
+          unfolding infinite_variables_per_type_def \<V>\<^sub>3_def if_distrib if_distribR Collect_if_eq 
+            Collect_not_mem_conj_eq
+          by auto
+      qed
+          
+      show "\<iota>\<^sub>G \<in> ground.G_Inf"
+        unfolding ground.G_Inf_def
+        using ground_superposition
+        by simp
+    qed
+  qed
+qed
+
+subsection \<open>Ground instances\<close>
+
+context
+  fixes \<iota>\<^sub>G N
+  assumes 
+    subst_stability: "subst_stability_on N" and
+    \<iota>\<^sub>G_Inf_from: "\<iota>\<^sub>G \<in> ground.Inf_from_q select\<^sub>G (\<Union>(clause_groundings ` N))" 
+begin
+
+lemma single_premise_ground_instance:
+  assumes 
+    ground_inference: "\<iota>\<^sub>G \<in>  {Infer [D] C | D C. ground_inference D C}" and
+    lifting: "\<And>D \<gamma> C \<V> thesis. \<lbrakk>
+    ground_inference (clause.to_ground (D \<cdot> \<gamma>)) (clause.to_ground (C \<cdot> \<gamma>)); 
+    clause.is_ground (D \<cdot> \<gamma>); 
+    clause.is_ground (C \<cdot> \<gamma>);
+    clause.from_ground (select\<^sub>G (clause.to_ground (D \<cdot> \<gamma>))) = select D \<cdot> \<gamma>; 
+    clause.is_welltyped \<V> D; is_welltyped_on (clause.vars D) \<V> \<gamma>;
+    infinite_variables_per_type \<V>;
+    \<And>C'. \<lbrakk>
+        inference (D, \<V>) (C', \<V>);
+        Infer [clause.to_ground (D \<cdot> \<gamma>)] (clause.to_ground (C \<cdot> \<gamma>))
+        \<in> inference_groundings (Infer [(D, \<V>)] (C', \<V>));
+        C' \<cdot> \<gamma> = C \<cdot> \<gamma>\<rbrakk> \<Longrightarrow> thesis\<rbrakk>
+       \<Longrightarrow> thesis" and
+    inference_eq: "inference = eq_factoring \<or> inference = eq_resolution"
+  obtains \<iota> where 
+    "\<iota> \<in> Inf_from N" 
+    "\<iota>\<^sub>G \<in> inference_groundings \<iota>"
+proof-
+  obtain D\<^sub>G C\<^sub>G where 
+    \<iota>\<^sub>G: "\<iota>\<^sub>G = Infer [D\<^sub>G] C\<^sub>G" and
+    ground_inference: "ground_inference D\<^sub>G C\<^sub>G"
+    using ground_inference
+    by blast
+
+  have D\<^sub>G_in_groundings: "D\<^sub>G \<in> \<Union>(clause_groundings ` N)"
+    using \<iota>\<^sub>G_Inf_from
+    unfolding \<iota>\<^sub>G ground.Inf_from_q_def ground.Inf_from_def
+    by simp
+
+  obtain D \<gamma> \<V> where
+    D_grounding: "clause.is_ground (D \<cdot> \<gamma>)" and
+    D_is_welltyped: "clause.is_welltyped \<V> D" and
+    \<gamma>_is_welltyped: "is_welltyped_on (clause.vars D) \<V> \<gamma>" and
+    \<V>: "infinite_variables_per_type \<V>" and
+    D_in_N: "(D, \<V>)\<in>N" and 
+    "select\<^sub>G D\<^sub>G = clause.to_ground (select D \<cdot> \<gamma>)"
+    "D \<cdot> \<gamma> = clause.from_ground D\<^sub>G"
+    using subst_stability[rule_format, OF D\<^sub>G_in_groundings]
+    by blast
+
+  then have 
+    D\<^sub>G: "D\<^sub>G = clause.to_ground (D \<cdot> \<gamma>)" and
+    select: "clause.from_ground (select\<^sub>G D\<^sub>G) = select D \<cdot> \<gamma>"
+    by (simp_all add: select_ground_subst)
+
+  obtain C where 
+    C\<^sub>G: "C\<^sub>G = clause.to_ground (C \<cdot> \<gamma>)" and 
+    C_grounding: "clause.is_ground (C \<cdot> \<gamma>)"
+    by (metis clause.all_subst_ident_iff_ground clause.from_ground_inverse 
+        clause.ground_is_ground)
+
+  obtain C' where 
+    inference: "inference (D, \<V>) (C', \<V>)" and
+    inference_groundings: "\<iota>\<^sub>G \<in> inference_groundings (Infer [(D, \<V>)] (C', \<V>))" and  
+    C'_C: "C' \<cdot> \<gamma> = C \<cdot> \<gamma>"
+    using
+      lifting[OF 
+        ground_inference[unfolded D\<^sub>G C\<^sub>G]
+        D_grounding
+        C_grounding
+        select[unfolded D\<^sub>G]
+        D_is_welltyped
+        \<gamma>_is_welltyped
+        \<V>]
+    unfolding D\<^sub>G C\<^sub>G \<iota>\<^sub>G.
+
+  let ?\<iota> = "Infer [(D, \<V>)] (C', \<V>)"
+
+  show ?thesis
+  proof(rule that[OF _ inference_groundings])
+
+    show "?\<iota> \<in> Inf_from N"
+      using D_in_N inference inference_eq
+      unfolding Inf_from_def inferences_def inference_system.Inf_from_def
+      by auto
+  qed
+qed
+
+lemma eq_resolution_ground_instance: 
+  assumes ground_eq_resolution: "\<iota>\<^sub>G \<in> ground.eq_resolution_inferences" 
+  obtains \<iota> where             
+    "\<iota> \<in> Inf_from N" 
+    "\<iota>\<^sub>G \<in> inference_groundings \<iota>"
+  using eq_resolution_lifting single_premise_ground_instance[OF ground_eq_resolution]
+  by blast
+  
+lemma eq_factoring_ground_instance: 
+  assumes ground_eq_factoring: "\<iota>\<^sub>G \<in> ground.eq_factoring_inferences" 
+  obtains \<iota> where 
+    "\<iota> \<in> Inf_from N" 
+    "\<iota>\<^sub>G \<in> inference_groundings \<iota>"
+  using eq_factoring_lifting single_premise_ground_instance[OF ground_eq_factoring]
+  by blast
+
+lemma superposition_ground_instance: 
+  assumes 
+    ground_superposition: "\<iota>\<^sub>G \<in> ground.superposition_inferences" and
+    not_redundant: "\<iota>\<^sub>G \<notin> ground.GRed_I (\<Union> (clause_groundings ` N))"
+  obtains \<iota> where 
+    "\<iota> \<in> Inf_from N" 
+    "\<iota>\<^sub>G \<in> inference_groundings \<iota>"
+proof-
+  obtain E\<^sub>G D\<^sub>G C\<^sub>G where 
+    \<iota>\<^sub>G : "\<iota>\<^sub>G = Infer [D\<^sub>G, E\<^sub>G] C\<^sub>G" and
+    ground_superposition: "ground.superposition D\<^sub>G E\<^sub>G C\<^sub>G"
+    using assms(1)
+    by blast
+
+  have 
+    E\<^sub>G_in_groundings: "E\<^sub>G \<in> \<Union> (clause_groundings ` N)" and  
+    D\<^sub>G_in_groundings: "D\<^sub>G \<in> \<Union> (clause_groundings ` N)"
+    using \<iota>\<^sub>G_Inf_from
+    unfolding \<iota>\<^sub>G ground.Inf_from_q_def ground.Inf_from_def
+    by simp_all
+
+  obtain E \<V>\<^sub>1 \<gamma>\<^sub>1 where
+    E_grounding: "clause.is_ground (E \<cdot> \<gamma>\<^sub>1)" and
+    E_is_welltyped: "clause.is_welltyped \<V>\<^sub>1 E" and
+    \<gamma>\<^sub>1_is_welltyped: "is_welltyped_on (clause.vars E) \<V>\<^sub>1 \<gamma>\<^sub>1" and
+    \<V>\<^sub>1: "infinite_variables_per_type \<V>\<^sub>1" and
+    E_in_N: "(E, \<V>\<^sub>1)\<in>N" and 
+    "select\<^sub>G E\<^sub>G = clause.to_ground (select E \<cdot> \<gamma>\<^sub>1)"
+    "E \<cdot> \<gamma>\<^sub>1 = clause.from_ground E\<^sub>G"
+    using subst_stability[rule_format, OF E\<^sub>G_in_groundings]
+    by blast
+
+  then have 
+    E\<^sub>G: "E\<^sub>G = clause.to_ground (E \<cdot> \<gamma>\<^sub>1)" and
+    select_from_E: "clause.from_ground (select\<^sub>G E\<^sub>G) = select E \<cdot> \<gamma>\<^sub>1"
+    by (simp_all add: select_ground_subst)
+
+  obtain D \<V>\<^sub>2 \<gamma>\<^sub>2 where
+    D_grounding: "clause.is_ground (D \<cdot> \<gamma>\<^sub>2)" and
+    D_is_welltyped: "clause.is_welltyped \<V>\<^sub>2 D" and
+    \<gamma>\<^sub>2_is_welltyped: "is_welltyped_on (clause.vars D) \<V>\<^sub>2 \<gamma>\<^sub>2" and
+    \<V>\<^sub>2: "infinite_variables_per_type \<V>\<^sub>2" and
+    D_in_N: "(D, \<V>\<^sub>2)\<in>N" and 
+    "select\<^sub>G D\<^sub>G = clause.to_ground (select D \<cdot> \<gamma>\<^sub>2)"
+    "D \<cdot> \<gamma>\<^sub>2 = clause.from_ground D\<^sub>G"
+    using subst_stability[rule_format, OF D\<^sub>G_in_groundings] 
+    by blast
+
+  then have 
+    D\<^sub>G: "D\<^sub>G = clause.to_ground (D \<cdot> \<gamma>\<^sub>2)" and
+    select_from_D: "clause.from_ground (select\<^sub>G D\<^sub>G) = select D \<cdot> \<gamma>\<^sub>2"
+    by (simp_all add: select_ground_subst)
+
+  obtain \<rho>\<^sub>1 \<rho>\<^sub>2 \<gamma> :: "('f, 'v) subst" where
+    \<rho>\<^sub>1: "term_subst.is_renaming \<rho>\<^sub>1" and
+    \<rho>\<^sub>2: "term_subst.is_renaming \<rho>\<^sub>2" and
+    rename_apart:  "clause.vars (E \<cdot> \<rho>\<^sub>1) \<inter> clause.vars (D \<cdot> \<rho>\<^sub>2) = {}" and
+    \<rho>\<^sub>1_is_welltyped: "is_welltyped_on (clause.vars E) \<V>\<^sub>1 \<rho>\<^sub>1" and
+    \<rho>\<^sub>2_is_welltyped: "is_welltyped_on (clause.vars D) \<V>\<^sub>2 \<rho>\<^sub>2" and
+    \<gamma>\<^sub>1_\<gamma>: "\<forall>X \<subseteq> clause.vars E. \<forall>x\<in> X. \<gamma>\<^sub>1 x = (\<rho>\<^sub>1 \<odot> \<gamma>) x" and
+    \<gamma>\<^sub>2_\<gamma>: "\<forall>X \<subseteq> clause.vars D. \<forall>x\<in> X. \<gamma>\<^sub>2 x = (\<rho>\<^sub>2 \<odot> \<gamma>) x"
+    using 
+      clause.finite_vars 
+      \<V>\<^sub>1 \<V>\<^sub>2
+      clause.is_welltyped.obtain_welltyped_merged_grounding[OF 
+        \<gamma>\<^sub>1_is_welltyped \<gamma>\<^sub>2_is_welltyped E_grounding D_grounding _ _ infinite_UNIV]
+    unfolding infinite_variables_per_type_def
+    by blast
+
+  have E_grounding: "clause.is_ground (E \<cdot> \<rho>\<^sub>1 \<odot> \<gamma>)"
+    using clause.subst_eq \<gamma>\<^sub>1_\<gamma> E_grounding
+    by fastforce
+
+  have E\<^sub>G: "E\<^sub>G = clause.to_ground (E \<cdot> \<rho>\<^sub>1 \<odot> \<gamma>)"
+    using clause.subst_eq \<gamma>\<^sub>1_\<gamma> E\<^sub>G
+    by fastforce
+
+  have D_grounding: "clause.is_ground (D \<cdot> \<rho>\<^sub>2 \<odot> \<gamma>)"
+    using clause.subst_eq \<gamma>\<^sub>2_\<gamma> D_grounding
+    by fastforce
+
+  have D\<^sub>G: "D\<^sub>G = clause.to_ground (D \<cdot> \<rho>\<^sub>2 \<odot> \<gamma>)"
+    using clause.subst_eq \<gamma>\<^sub>2_\<gamma> D\<^sub>G
+    by fastforce
+
+  have \<rho>\<^sub>1_\<gamma>_is_welltyped: "is_welltyped_on (clause.vars E) \<V>\<^sub>1 (\<rho>\<^sub>1 \<odot> \<gamma>)"
+    using \<gamma>\<^sub>1_is_welltyped \<gamma>\<^sub>1_\<gamma>
+    by fastforce
+
+  have \<rho>\<^sub>2_\<gamma>_is_welltyped: "is_welltyped_on (clause.vars D) \<V>\<^sub>2 (\<rho>\<^sub>2 \<odot> \<gamma>)"
+    using \<gamma>\<^sub>2_is_welltyped \<gamma>\<^sub>2_\<gamma>
+    by fastforce
+
+  have select_vars_subset: "\<And>C. clause.vars (select C) \<subseteq> clause.vars C"
+    by (simp add: clause_submset_vars_clause_subset select_subset)
+
+  have select_from_E:
+    "clause.from_ground (select\<^sub>G (clause.to_ground (E \<cdot> \<rho>\<^sub>1 \<odot> \<gamma>))) = select E \<cdot> \<rho>\<^sub>1 \<odot> \<gamma>"
+  proof-
+    have "E \<cdot> \<gamma>\<^sub>1 = E \<cdot> \<rho>\<^sub>1 \<odot> \<gamma>"
+      using \<gamma>\<^sub>1_\<gamma> clause.subst_eq
+      by fast
+
+    moreover have "select E \<cdot> \<gamma>\<^sub>1 = select E \<cdot> \<rho>\<^sub>1 \<cdot> \<gamma>"
+      using clause.subst_eq \<gamma>\<^sub>1_\<gamma> select_vars_subset
+      by (metis clause.comp_subst.left.monoid_action_compatibility)
+
+    ultimately show ?thesis
+      using select_from_E
+      unfolding E\<^sub>G
+      by simp
+  qed
+
+  have select_from_D:
+    "clause.from_ground (select\<^sub>G (clause.to_ground (D \<cdot> \<rho>\<^sub>2 \<odot> \<gamma>))) = select D \<cdot> \<rho>\<^sub>2 \<odot> \<gamma>"
+  proof-   
+    have "D \<cdot> \<gamma>\<^sub>2 = D \<cdot> \<rho>\<^sub>2 \<odot> \<gamma>"
+      using \<gamma>\<^sub>2_\<gamma> clause.subst_eq
+      by fast
+
+    moreover have "select D \<cdot> \<gamma>\<^sub>2 = select D \<cdot> \<rho>\<^sub>2 \<cdot> \<gamma>"
+      using clause.subst_eq \<gamma>\<^sub>2_\<gamma> select_vars_subset
+      by (metis clause.comp_subst.left.monoid_action_compatibility)
+
+    ultimately show ?thesis
+      using select_from_D
+      unfolding D\<^sub>G
+      by simp
+  qed
+
+  obtain C where
+    C_grounding: "clause.is_ground (C \<cdot> \<gamma>)" and
+    C\<^sub>G: "C\<^sub>G = clause.to_ground (C \<cdot> \<gamma>)"
+    by (metis clause.all_subst_ident_if_ground clause.from_ground_inverse clause.ground_is_ground)
+
+  have "clause_groundings (E, \<V>\<^sub>1) \<union> clause_groundings (D, \<V>\<^sub>2) \<subseteq> \<Union> (clause_groundings ` N)"
+    using E_in_N D_in_N 
+    by blast
+
+  then have \<iota>\<^sub>G_not_redundant:
+    "\<iota>\<^sub>G \<notin> ground.GRed_I (clause_groundings (E, \<V>\<^sub>1) \<union> clause_groundings (D, \<V>\<^sub>2))"
+    using not_redundant ground.Red_I_of_subset
+    by blast
+
+  obtain C' \<V>\<^sub>3 where 
+    superposition: "superposition (D, \<V>\<^sub>2) (E, \<V>\<^sub>1) (C', \<V>\<^sub>3)" and
+    inference_groundings: "\<iota>\<^sub>G \<in> inference_groundings (Infer [(D, \<V>\<^sub>2), (E, \<V>\<^sub>1)] (C', \<V>\<^sub>3))" and  
+    C'_\<gamma>_C_\<gamma>: "C' \<cdot> \<gamma> = C \<cdot> \<gamma>"
+    using 
+      superposition_lifting[OF 
+        ground_superposition[unfolded D\<^sub>G E\<^sub>G C\<^sub>G]
+        \<rho>\<^sub>1 \<rho>\<^sub>2
+        rename_apart
+        E_grounding D_grounding C_grounding
+        select_from_E select_from_D
+        E_is_welltyped D_is_welltyped
+        \<rho>\<^sub>1_\<gamma>_is_welltyped \<rho>\<^sub>2_\<gamma>_is_welltyped
+        \<rho>\<^sub>1_is_welltyped \<rho>\<^sub>2_is_welltyped
+        \<V>\<^sub>1 \<V>\<^sub>2
+        \<iota>\<^sub>G_not_redundant[unfolded \<iota>\<^sub>G D\<^sub>G E\<^sub>G C\<^sub>G]
+        ]
+    unfolding \<iota>\<^sub>G C\<^sub>G E\<^sub>G D\<^sub>G .
+
+  let ?\<iota> = "Infer [(D, \<V>\<^sub>2), (E, \<V>\<^sub>1)] (C', \<V>\<^sub>3)"
+
+  show ?thesis
+  proof(rule that[OF _ inference_groundings])
+
+    show "?\<iota> \<in> Inf_from N"
+      using E_in_N D_in_N superposition
+      unfolding Inf_from_def inferences_def inference_system.Inf_from_def
+      by auto
+  qed
+qed  
+
+lemma ground_instances: 
+  assumes not_redundant: "\<iota>\<^sub>G \<notin> ground.Red_I (\<Union> (clause_groundings ` N))"
+  obtains \<iota> where 
+    "\<iota> \<in> Inf_from N" 
+    "\<iota>\<^sub>G \<in> inference_groundings \<iota>"
+proof-
+  consider 
+    (superposition) "\<iota>\<^sub>G \<in> ground.superposition_inferences" |
+    (eq_resolution) "\<iota>\<^sub>G \<in> ground.eq_resolution_inferences" |
+    (eq_factoring) "\<iota>\<^sub>G \<in> ground.eq_factoring_inferences"
+    using \<iota>\<^sub>G_Inf_from
+    unfolding
+      ground.Inf_from_q_def 
+      ground.G_Inf_def
+      inference_system.Inf_from_def
+    by fastforce
+
+  then show ?thesis
+  proof cases
+    case superposition
+
+    then show ?thesis
+      using that superposition_ground_instance not_redundant
+      by blast
+  next
+    case eq_resolution
+
+    then show ?thesis
+      using that eq_resolution_ground_instance
+      by blast
+  next
+    case eq_factoring
+
+    then show ?thesis
+      using that eq_factoring_ground_instance
+      by blast
+  qed
+qed
+
+end
+
+end
+
+context superposition_calculus
+begin
+
+lemma overapproximation:
+  obtains select\<^sub>G where
+    "ground_Inf_overapproximated select\<^sub>G premises"
+    "is_grounding select\<^sub>G"
+proof-
+  obtain select\<^sub>G where   
+    subst_stability: "select_subst_stability_on select select\<^sub>G premises" and
+    "is_grounding select\<^sub>G"
+    using obtain_subst_stable_on_select_grounding
+    by blast
+
+  then interpret grounded_superposition_calculus
+    where select\<^sub>G = select\<^sub>G
+    by unfold_locales
+
+  show thesis
+  proof(rule that[OF _ select\<^sub>G])
+
+    show "ground_Inf_overapproximated select\<^sub>G premises"
+      using ground_instances[OF subst_stability]
+      by auto
+  qed
+qed
+
+sublocale statically_complete_calculus "\<bottom>\<^sub>F" inferences entails_\<G> Red_I_\<G> Red_F_\<G>
+proof(unfold static_empty_ord_inter_equiv_static_inter, 
+    rule stat_ref_comp_to_non_ground_fam_inter, 
+    rule ballI)
+  fix select\<^sub>G
+  assume "select\<^sub>G \<in> select\<^sub>G\<^sub>s"
+  then interpret grounded_superposition_calculus
+    where select\<^sub>G = select\<^sub>G
+    by unfold_locales (simp add: select\<^sub>G\<^sub>s_def)
+
+  show "statically_complete_calculus
+          ground.G_Bot
+          ground.G_Inf
+          ground.G_entails
+          ground.Red_I
+          ground.Red_F"
+    using ground.statically_complete_calculus_axioms.
+next
+
+  show "\<And>N. \<exists>select\<^sub>G \<in> select\<^sub>G\<^sub>s. ground_Inf_overapproximated select\<^sub>G N" 
+    using overapproximation
+    unfolding select\<^sub>G\<^sub>s_def
+    by (smt (verit, best) mem_Collect_eq)
+qed
+
+end
+
+end
