thys/Superposition_Calculus/Typing.thy
@@ -1,0 +1,112 @@
+theory Typing
+  imports Main
+begin
+
+locale typing =
+  fixes is_typed is_welltyped
+  assumes is_typed_if_is_welltyped: 
+    "\<And>expr. is_welltyped expr \<Longrightarrow> is_typed expr"
+
+(* TODO: Should not be a locale *)
+locale predicate_typed = 
+  fixes typed :: "'expr \<Rightarrow> 'ty \<Rightarrow> bool"
+  assumes right_unique: "right_unique typed"
+begin
+
+abbreviation is_typed where
+  "is_typed expr \<equiv> \<exists>\<tau>. typed expr \<tau>"
+
+lemmas right_uniqueD [dest] = right_uniqueD[OF right_unique] 
+
+end
+
+locale explicit_typing =
+  typed: predicate_typed where typed = typed +
+  welltyped: predicate_typed where typed = welltyped
+for typed welltyped :: "'expr \<Rightarrow> 'ty \<Rightarrow> bool" +
+assumes typed_if_welltyped: "\<And>expr \<tau>. welltyped expr \<tau> \<Longrightarrow> typed expr \<tau>"
+begin
+
+abbreviation is_typed where
+  "is_typed \<equiv> typed.is_typed"
+
+abbreviation is_welltyped where
+  "is_welltyped \<equiv> welltyped.is_typed"
+
+sublocale typing where is_typed = is_typed and is_welltyped = is_welltyped
+   using typed_if_welltyped
+   by unfold_locales auto
+
+(* TODO: Name *)
+lemma typed_welltyped:
+  assumes "typed expr \<tau>" "welltyped expr \<tau>'"
+  shows "welltyped expr \<tau>"
+  using assms typed_if_welltyped
+  by blast
+
+end
+
+definition uniform_typed_lifting where 
+  "uniform_typed_lifting to_set sub_typed expr \<equiv> \<exists>\<tau>. \<forall>sub \<in> to_set expr. sub_typed sub \<tau>"
+
+definition is_typed_lifting where 
+  "is_typed_lifting to_set sub_is_typed expr \<equiv> \<forall>sub \<in> to_set expr. sub_is_typed sub"
+
+locale uniform_typing_lifting = 
+  sub: explicit_typing where typed = sub_typed and welltyped = sub_welltyped
+for sub_typed sub_welltyped :: "'sub \<Rightarrow> 'ty \<Rightarrow> bool" +
+fixes to_set :: "'expr \<Rightarrow> 'sub set"
+begin
+
+abbreviation is_typed where
+  "is_typed \<equiv> uniform_typed_lifting to_set sub_typed"
+
+lemmas is_typed_def = uniform_typed_lifting_def[of to_set sub_typed]
+
+abbreviation is_welltyped where
+  "is_welltyped \<equiv> uniform_typed_lifting to_set sub_welltyped"
+  
+lemmas is_welltyped_def = uniform_typed_lifting_def[of to_set sub_welltyped]
+
+sublocale typing where is_typed = is_typed and is_welltyped = is_welltyped
+proof unfold_locales
+  fix expr
+  assume "is_welltyped expr"  
+  then show "is_typed expr"
+    using sub.typed_if_welltyped
+    unfolding is_typed_def is_welltyped_def
+    by auto
+qed
+
+end
+
+locale typing_lifting =
+  sub: typing where is_typed = sub_is_typed and is_welltyped = sub_is_welltyped
+for sub_is_typed sub_is_welltyped :: "'sub \<Rightarrow> bool" +
+fixes 
+  to_set :: "'expr \<Rightarrow> 'sub set"
+begin
+
+abbreviation is_typed where
+  "is_typed \<equiv> is_typed_lifting to_set sub_is_typed"
+
+lemmas is_typed_def = is_typed_lifting_def[of to_set sub_is_typed]
+
+abbreviation is_welltyped where
+  "is_welltyped \<equiv> is_typed_lifting to_set sub_is_welltyped"
+
+lemmas is_welltyped_def = is_typed_lifting_def[of to_set sub_is_welltyped]
+
+sublocale typing where is_typed = is_typed and is_welltyped = is_welltyped
+proof unfold_locales
+  fix expr
+  assume "is_welltyped expr"
+  then show "is_typed expr"
+    using sub.is_typed_if_is_welltyped
+    unfolding is_typed_def is_welltyped_def
+    by simp
+qed
+
+end
+
+end
